wip

Matroid/Extremal/Covers.lean
@@ -34,10 +34,10 @@ structure Set.IsCover (T : Set (Set α)) (X : Set α) (P : Set α → Prop) : Pr
 lemma Set.IsCover.subset (h : T.IsCover X P) (hY : Y ∈ T) : Y ⊆ X := by
   grw [← h.sUnion_eq, ← subset_sUnion_of_mem hY]
 
-def Set.hasCover_with (X : Set α) (P : Set α → Prop) : Prop :=
+def Set.hasCover (X : Set α) (P : Set α → Prop) : Prop :=
     ∃ T, IsCover T X P
 
-lemma Cover_Nonempt_iff {X : Set α} : X.hasCover_with P ↔ {T | IsCover T X P }.Nonempty := Iff.rfl
+lemma hasCover_iff {X : Set α} : X.hasCover P ↔ {T | IsCover T X P }.Nonempty := Iff.rfl
 
 lemma Set.IsCover.nonempty (h : T.IsCover X P) (hX : X.Nonempty) : T.Nonempty := by
   rw [nonempty_iff_empty_ne]
@@ -45,9 +45,9 @@ lemma Set.IsCover.nonempty (h : T.IsCover X P) (hX : X.Nonempty) : T.Nonempty :=
   simp [isCover_iff, eq_comm] at h
   simp_all only [Set.not_nonempty_empty]
 
-lemma IsCover.one_le (h : T.IsCover X P ) (hX : X.Nonempty) : T.Nonempty := by
-  --simp only [one_le_encard_iff_nonempty]
-  exact h.nonempty hX
+-- lemma IsCover.one_le (h : T.IsCover X P ) (hX : X.Nonempty) : T.Nonempty := by
+--   --simp only [one_le_encard_iff_nonempty]
+--   exact h.nonempty hX
 
 lemma isCover_iff_isCover_subset : T.IsCover X P ↔ T.IsCover X (fun A ↦ P A ∧ A ⊆ X) := by
   rw [isCover_iff, isCover_iff]
@@ -62,18 +62,9 @@ lemma isCover_iff_isCover_subset : T.IsCover X P ↔ T.IsCover X (fun A ↦ P A 
     rcases hAPsub F hF with ⟨hPF, hFX⟩
     exact hPF
 
--- --Monotono subset
--- def IsMRProp (P : Set α → Prop) : Prop :=
---     ∀ F : Set α, ∀ Y : Set α, Y ⊆ F → P Y → P F
-
--- -- def IsMRProp (P : Matroid α → Set α → Prop) : Prop :=
--- --     ∀ M : Matroid α, ∀ F : Set α, ∀ Y : Set α, Y ⊆ F → P (M ↾ F) Y → P M Y
-
--- --Monotone under subset
--- def IsMSProp (P : Set α → Prop) : Prop :=
---     ∀ F : Set α, ∀ Y : Set α, Y ⊆ F → P F → P Y
-
-lemma IsCover.cover_typset {E : Set α}
+/-- The covers of each element of a cover define a cover.
+In this case we use typesets to give the cover of covers-/
+lemma Set.IsCover.biUnion' {E : Set α}
     (hcover : T.IsCover E P )
     (f : T → Set (Set α) )
     (hfun : ∀ X : T, (f X).IsCover X.1 P' ) :
@@ -92,7 +83,6 @@ lemma IsCover.cover_typset {E : Set α}
     simp only [mem_sUnion] at he
     obtain ⟨X, hXT, heX⟩ := he
     simp only [iUnion_coe_set, mem_sUnion, mem_iUnion]
-    --have h1 : e ∈ ↑X := by exact mem_of_subset_of_mem (fun ⦃a⦄ a_1 ↦ a_1) heX
     have h1 := (hfun ⟨X, hXT⟩ ).sUnion_eq
     simp only at h1
     rw[←h1] at heX
@@ -103,9 +93,9 @@ lemma IsCover.cover_typset {E : Set α}
   simp only [iUnion_coe_set, mem_iUnion] at hF
   obtain ⟨X, hXT, hF⟩ := hF
   exact (hfun ⟨X, hXT⟩).pProp F hF
-  --exact hP' X F (LE.le.subset ((hfun ⟨X, hXT⟩).subset_ground hF ) ) ((hfun ⟨X, hXT⟩).pProp F hF)
 
-lemma Set.IsCover.cover_fun {P' :  Set α → Prop}
+/-- The covers of each element of a cover define a cover. -/
+lemma Set.IsCover.biUnion {P' :  Set α → Prop}
     (hcover : T.IsCover Y P )
     (f : Set α → Set (Set α) )
     (hfun : ∀ X ∈ T, (f X).IsCover X P' ) :
@@ -124,7 +114,6 @@ lemma Set.IsCover.cover_fun {P' :  Set α → Prop}
     simp only [mem_sUnion] at he
     obtain ⟨X, hXT, heX⟩ := he
     simp only [mem_sUnion, mem_iUnion]
-    --have h1 : e ∈ (M ↾ ↑X).E := by exact mem_of_subset_of_mem (fun ⦃a⦄ a_1 ↦ a_1) heX
     have h1 := (hfun X hXT ).sUnion_eq
     rw[←(hfun X hXT ).sUnion_eq] at heX
     simp only [mem_sUnion] at heX
@@ -134,12 +123,11 @@ lemma Set.IsCover.cover_fun {P' :  Set α → Prop}
   simp only [ mem_iUnion] at hF
   obtain ⟨X, hXT, hF⟩ := hF
   exact (hfun X hXT).pProp F hF
-  --exact hP' M X F (LE.le.subset ((hfun X hXT).subset_ground hF ) ) ((hfun X hXT).pProp F hF)
 
 lemma IsCover.mono_prop (h : T.IsCover Y P ) (hPP' : ∀ X ∈ T, P X → P' X) : T.IsCover Y P' :=
   (T.isCover_iff Y P').2 ⟨h.sUnion_eq, fun F hF ↦ hPP' F hF (h.pProp F hF)⟩
 
-lemma IsCover_emptyset_iff (P : Set α → Prop) : IsCover ∅ Y P ↔ Y = ∅ := by
+lemma isCover_empty_iff (P : Set α → Prop) : IsCover ∅ Y P ↔ Y = ∅ := by
   refine ⟨?_, ?_ ⟩
   · intro h
     rw [ ←sUnion_empty, h.sUnion_eq.symm ]
@@ -147,7 +135,8 @@ lemma IsCover_emptyset_iff (P : Set α → Prop) : IsCover ∅ Y P ↔ Y = ∅ :
   rw [ ←sUnion_empty] at h
   refine ⟨h.symm, by grind ⟩
 
-lemma Set.IsCover.contract (h : T.IsCover Y P)
+--Peter, is this a better name?
+lemma Set.IsCover.image_union (h : T.IsCover Y P)
     (hXN : Y.Nonempty)
     (hPP' : ∀ F : Set α, P F → P' ( F ∪ X) ) :
     ((· ∪ X) '' T).IsCover (Y ∪ X) P' := by
@@ -155,12 +144,10 @@ lemma Set.IsCover.contract (h : T.IsCover Y P)
     simp only [isCover_iff, sUnion_image, mem_image, forall_exists_index, and_imp,
       forall_apply_eq_imp_iff₂, ← biUnion_distrib_union _ (h.nonempty hXN), ← sUnion_eq_biUnion,
       h.sUnion_eq, true_and  ]
-      --  ← biUnion_distrib_union _ h.nonempty, ← sUnion_eq_biUnion,
-      -- h.sUnion_eq, contract_ground, diff_union_self, union_eq_left, hX, true_and ]
     exact fun F hFT ↦ (((fun a ↦ (hPP' F (hi F hFT))) ∘ T) X )
   exact fun F hFT ↦ h.pProp F hFT
 
-lemma Set.IsCover.mono_set (h : T.IsCover X P ) (hX : Y ⊆ X)
+lemma Set.IsCover.mono_subset (h : T.IsCover X P ) (hX : Y ⊆ X)
     (hp : ∀ Z, P Z → P (Z ∩ Y) )
     : ((· ∩ Y) '' T).IsCover Y P := by
   refine ⟨?_, ?_ ⟩
@@ -176,7 +163,8 @@ lemma Set.IsCover.mono_set (h : T.IsCover X P ) (hX : Y ⊆ X)
   simp only
   exact hp Z (h.pProp Z hZ)
 
-lemma Set.IsCover.unionIsCover (T : Set (Set α)) (P : Set α → Prop) (hF : ∀ F ∈ T, P F) :
+--Not sure about name
+lemma Set.isCover_union (T : Set (Set α)) (P : Set α → Prop) (hF : ∀ F ∈ T, P F) :
     T.IsCover ( ⋃ F ∈ T, F ) P := by
   refine ⟨sUnion_eq_biUnion, fun F hF' ↦ hF F hF' ⟩
 
@@ -184,7 +172,7 @@ end General
 
 section Number
 
-/-- Docstring here -/
+/-- This is the size of the smallest cover -/
 noncomputable def Set.coverNumber (X : Set α) (P : Set α → Prop) : ℕ∞ :=
   ⨅ (T : Set (Set α)) (_ : T.IsCover X P), T.encard
 
@@ -197,10 +185,10 @@ lemma coverNumber_mono (X : Set α) {P Q : Set α → Prop} (hPQ : ∀ Y ⊆ X, 
 
 lemma Set.IsCover.coverNumber_le {T : Set (Set α)} (h : T.IsCover X P ) :
     X.coverNumber P ≤ T.encard := by
-  simp only [coverNumber, ]
+  simp only [coverNumber ]
   exact biInf_le encard h
 
-lemma exists_mincover_NE {P : Set α → Prop}
+lemma encard_eq_coverNumber_of_nonempty {P : Set α → Prop}
     (hn : {T | IsCover T X P }.Nonempty) :
     ∃ T, IsCover T X P ∧ T.encard = X.coverNumber P := by
   simp only [coverNumber]
@@ -210,9 +198,9 @@ lemma exists_mincover_NE {P : Set α → Prop}
   refine ⟨T.1, ⟨T.2, hT ⟩ ⟩
   -- have := ENat.exists_eq_iInf (f := fun (hT : T.IsCover X P) ↦ T.encard)
 
-lemma exists_min_cover (hP : X.hasCover_with P) :
+lemma exists_encard_eq_coverNumber (hP : X.hasCover P) :
     ∃ T, IsCover T X P ∧ T.encard = X.coverNumber P := by
-  exact exists_mincover_NE hP
+  exact encard_eq_coverNumber_of_nonempty hP
 
 lemma Set.exists_cover (X : Set α ) (P : Set α → Prop) :
     X.coverNumber P = ⊤ ∨ ∃ T, IsCover T X P ∧ T.encard = X.coverNumber P := by
@@ -225,9 +213,9 @@ lemma Set.exists_cover (X : Set α ) (P : Set α → Prop) :
     by_contra
     exact Ne.elim (ne_of_mem_of_not_mem' hT fun a ↦ a ) h0
   right
-  exact exists_min_cover h
+  exact exists_encard_eq_coverNumber h
 
-lemma coverNumber_positive (hX : X.Nonempty) (P : Set α → Prop) : 1 ≤ X.coverNumber P := by
+lemma one_le_coverNumber (hX : X.Nonempty) (P : Set α → Prop) : 1 ≤ X.coverNumber P := by
   by_contra hc
   have h1 := ENat.lt_one_iff_eq_zero.mp (Std.not_le.mp hc)
   obtain ht | ⟨T, hT, hTe ⟩ := X.exists_cover P
@@ -236,10 +224,11 @@ lemma coverNumber_positive (hX : X.Nonempty) (P : Set α → Prop) : 1 ≤ X.cov
   have : T.Nonempty := hT.nonempty hX
   grind
 
-/-- Docstring
-call it `coverNumber_le_tsum_coverNumber`?
+/--
+Given a cover we can bound the cover number with the cover number of each element of the cover.
+See IsCover.biUnion'
 -/
-lemma coverNumber_cover_of_covers {P' : Set α → Prop} (hcover : T.IsCover Y P ) :
+lemma coverNumber_le_tsum_coverNumber {P' : Set α → Prop} (hcover : T.IsCover Y P ) :
     Y.coverNumber P' ≤ ∑' X : T, (X.1).coverNumber P' := by
   obtain (h0 | h1) := exists_or_forall_not (fun X : T ↦ coverNumber X P' = ⊤)
   · simp [ENat.tsum_eq_top_of_eq_top h0]
@@ -250,21 +239,21 @@ lemma coverNumber_cover_of_covers {P' : Set α → Prop} (hcover : T.IsCover Y P
     · simp [h1 _ h]
     exact ⟨XT, hXres, hencard⟩
   choose f hfunco hfunca using hf
-  have hcover := IsCover.cover_typset hcover f hfunco
+  have hcover := IsCover.biUnion' hcover f hfunco
   grw [hcover.coverNumber_le, ENat.encard_iUnion_le_tsum_encard, tsum_congr hfunca]
 
 
-lemma coverNumber_cover_of_covers_bound {P' : Set α → Prop} {k : ℕ∞}
+lemma coverNumber_le_bound {P' : Set α → Prop} {k : ℕ∞}
     (hcover : T.IsCover Y P)
     (hflat : ∀ F, P F → F.coverNumber P' ≤ k) :
     Y.coverNumber P' ≤ (T.encard) * k := by
-  grw [coverNumber_cover_of_covers hcover, ENat.tsum_le_tsum (g := fun _ ↦ k),
+  grw [coverNumber_le_tsum_coverNumber hcover, ENat.tsum_le_tsum (g := fun _ ↦ k),
     ENat.tsum_subtype_const, mul_comm]
   intro F
   simp [hflat _ <| hcover.pProp F F.2 ]
   --exact hP'
 
-lemma IsCover_singleton_Prop (hP : ∀ e ∈ X, P {e}) : (singleton '' X).IsCover X P  := by
+lemma isCover_image_singleton (hP : ∀ e ∈ X, P {e}) : (singleton '' X).IsCover X P  := by
   refine ⟨ ?_, ?_ ⟩
   · refine Eq.symm (ext ?_)
     intro x
@@ -280,12 +269,12 @@ lemma IsCover_singleton_Prop (hP : ∀ e ∈ X, P {e}) : (singleton '' X).IsCove
   rw[←heF]
   exact hP e heE
 
-lemma IsCover_singleton_le (hP : ∀ e ∈ X, P {e}) : X.coverNumber P ≤ X.encard := by
-  grw [(IsCover_singleton_Prop hP).coverNumber_le ]
+lemma isCover_singleton_le (hP : ∀ e ∈ X, P {e}) : X.coverNumber P ≤ X.encard := by
+  grw [(isCover_image_singleton hP).coverNumber_le ]
   set Sing : Set (Set α ) := { singleton e | e ∈ X} with hs
   exact encard_image_le singleton X
 
-lemma coverNumber_zero_iff (P : Set α → Prop) : X.coverNumber P = 0 ↔ IsCover ∅ X P := by
+lemma coverNumber_eq_zero_iff (P : Set α → Prop) : X.coverNumber P = 0 ↔ IsCover ∅ X P := by
   refine ⟨?_, ?_ ⟩
   · intro h
     obtain ht | ⟨T, hT, hTe ⟩ := exists_cover X P
@@ -316,28 +305,17 @@ lemma coverNumber_congr (P Q : Set α → Prop)
 
 end Number
 
-
-
--- def IsCCProp (α) (P : Matroid α → Set α → Prop) : Prop :=
---     ∀ M : Matroid α, ∀ F : Set α, P M F → P M (M.closure F)
-
--- lemma IsCover.isCover_closure (h : M.IsCover P T) (hP : IsCCProp α P) :
---     M.IsCover P (M.closure '' T) := by
---   simp only [isCover_iff, sUnion_image, subset_antisymm_iff (b := M.E), iUnion_subset_iff,
---     M.closure_subset_ground, implies_true, true_and, mem_image, forall_exists_index, and_imp,
---     forall_apply_eq_imp_iff₂]
---   grw [h.sUnion_eq.symm.subset, sUnion_eq_biUnion]
---   refine  ⟨biUnion_mono rfl.subset fun X hX ↦ M.subset_closure X (h.subset_ground hX),
---   fun F hF ↦ (hP M F (h.pProp F hF)) ⟩
 namespace Matroid
 section Matroid
 
-/-- Docstring here -/
-def IsCCProp (P : Matroid α → Set α → Prop) : Prop :=
-    ∀ M : Matroid α, ∀ F : Set α, P M F → P M (M.closure F)
+-- /-- Docstring here -/
+-- def IsCCProp (P : Matroid α → Set α → Prop) : Prop :=
+--     ∀ M : Matroid α, ∀ F : Set α, P M F → P M (M.closure F)
 
+/-- If a property is closed under closure, you can also look at the closure of a cover. -/
 lemma Set.IsCover.isCover_closure {P : Matroid α → Set α → Prop} {M : Matroid α}
-    (h : T.IsCover X (P M)) (hP : IsCCProp P) (hXc : M.IsFlat X) (hX : X ⊆ M.E) :
+    (h : T.IsCover X (P M)) (hP : ∀ F : Set α, P M F → P M (M.closure F))
+    (hXc : M.IsFlat X) (hX : X ⊆ M.E) :
     (M.closure '' T).IsCover X (P M) := by
   simp only [isCover_iff, sUnion_image, mem_image, forall_exists_index, and_imp,
     forall_apply_eq_imp_iff₂, subset_antisymm_iff (b := X), iUnion_subset_iff, mem_image,
@@ -345,58 +323,48 @@ lemma Set.IsCover.isCover_closure {P : Matroid α → Set α → Prop} {M : Matr
   nth_rw 1 [←M.isFlat_iff_closure_self.1 hXc ]
   refine ⟨⟨fun T' hT' ↦ closure_subset_closure_of_subset_closure
     (by simp only [M.isFlat_iff_closure_self.1 hXc,IsCover.subset h hT' ]) , ?_ ⟩,
-    fun F hF ↦ (hP M F (h.pProp F hF)) ⟩
+    fun F hF ↦ (hP F (h.pProp F hF)) ⟩
   · grw [h.sUnion_eq.symm.subset, sUnion_eq_biUnion]
     refine biUnion_mono rfl.subset fun Z hZ ↦ (subset_closure_iff_forall_subset_isFlat Z
       (LE.le.subset fun ⦃a⦄ a_1 ↦ hX ((IsCover.subset h hZ ) a_1) )).mpr fun F a a_1 ↦ a_1
 
--- lemma Set.IsCover.isCover_closure {P : Matroid α → Set α → Prop} {M :Matroid α }
---     (h : T.IsCover X (P M)) (hP : IsCCProp P) :
---     (M.closure '' T).IsCover (M.closure X) (P M) := by
---   simp only [isCover_iff, sUnion_image, mem_image, forall_exists_index, and_imp,
---     forall_apply_eq_imp_iff₂, mem_image,
---     forall_exists_index, and_imp, forall_apply_eq_imp_iff₂]
---   refine ⟨ ?_, ?_ ⟩
---   · apply subset_antisymm_iff.2 ?_
---     simp only [iUnion_subset_iff]
---     refine ⟨fun T' hT' ↦ (closure_subset_closure M (h.subset hT')), ?_ ⟩
---     rw [←h.sUnion_eq]
-
---     sorry
---   sorry
-
-
--- lemma coverNumber_mono_prop (P : Set α → Prop) {M N : Matroid α} (hMN : M.E = N.E)
---     (hMP : ∀ X ⊆ M.E, P N X → P M X) : M.coverNumber P ≤ N.coverNumber P := by
-
-
 end Matroid
 
 section Rank
+-- h.trans h'
+-- Nonspanning
 
-/-- Docstring here -/
+/-- Cover when the property is bounded rank. -/
 def IsRankCover (M : Matroid α) (T : Set (Set α)) (X : Set α) (k : ℕ∞) : Prop :=
     T.IsCover X (fun A ↦ M.eRk A ≤ k)
+
+/-- Cover number for Rank -/
+noncomputable def coverNumberByRank (M : Matroid α) (X : Set α) (k : ℕ∞) : ℕ∞ :=
+  X.coverNumber (fun A ↦ M.eRk A ≤ k)
 
 lemma IsRankCover.contract (h : (M ／ X).IsRankCover T Y k )
     (hXN : Y.Nonempty) :
     M.IsRankCover ((· ∪ X) '' T) (Y ∪ X) (k + M.eRk X)  := by
   unfold IsRankCover
   unfold IsRankCover at h
-  apply IsCover.contract h hXN
+  apply IsCover.image_union h hXN
   intro F hF
   rw [← @eRelRk_add_eRk_eq, eRelRk_eq_eRk_contract]
   exact add_le_add_left hF (M.eRk X)
 
-lemma IsRankCover_iff_IsCover {M : Matroid α} {T : Set (Set α)} {X : Set α} {k : ℕ∞} :
+lemma IsRankCover_iff {M : Matroid α} {T : Set (Set α)} {X : Set α} {k : ℕ∞} :
     M.IsRankCover T X k ↔ T.IsCover X (fun A ↦ M.eRk A ≤ k) := Iff.rfl
 
-lemma IsRankCover_iff (M : Matroid α) (T : Set (Set α)) (X : Set α) (k : ℕ∞) :
+lemma coverNumberByRank_eq {M : Matroid α} {X : Set α} {k : ℕ∞} :
+    M.coverNumberByRank X k = X.coverNumber (fun A ↦ M.eRk A ≤ k) := by
+  sorry
+
+lemma IsRankCover_iff' (M : Matroid α) (T : Set (Set α)) (X : Set α) (k : ℕ∞) :
     M.IsRankCover T X k ↔ ⋃₀ T = X ∧ (∀ F ∈ T, M.eRk F ≤ k) := by
-  rw [IsRankCover_iff_IsCover, isCover_iff]
+  rw [IsRankCover_iff, isCover_iff]
 
 lemma IsRankCover_iff_restriction : M.IsRankCover T X k ↔ (M ↾ X).IsRankCover T (M ↾ X).E k := by
-  rw [IsRankCover_iff, IsRankCover_iff, M.restrict_ground_eq]
+  rw [IsRankCover_iff', IsRankCover_iff', M.restrict_ground_eq]
   refine and_congr_right fun hU => ?_
   refine ⟨?_, ?_⟩
   · intro hRM F hFT
@@ -411,30 +379,20 @@ lemma IsRankCover_iff_restriction : M.IsRankCover T X k ↔ (M ↾ X).IsRankCove
     simpa [M.restrict_eRk_eq hFX] using hRMX F hFT
 
 lemma IsRankCover.subset (h : M.IsRankCover T X k) (hY : Y ∈ T) : Y ⊆ X :=
-  (IsRankCover_iff_IsCover.1 h ).subset hY
+  (IsRankCover_iff.1 h ).subset hY
 
 lemma IsRankCover.subset_ground (h : M.IsRankCover T X k) (hY : Y ∈ T)
-    (hX : X ⊆ M.E := by aesop_mat) : Y ⊆ M.E :=
-  LE.le.subset fun ⦃a⦄ a_1 ↦ hX (((IsRankCover_iff_IsCover.1 h ).subset hY ) a_1)
+    (hX : X ⊆ M.E := by aesop_mat) : Y ⊆ M.E := ((IsRankCover_iff.1 h ).subset hY).trans hX
 
-lemma IsRankCover.mono_set (hcov : M.IsRankCover T X k) (hX : Y ⊆ X) :
+lemma IsRankCover.mono_subset (hcov : M.IsRankCover T X k) (hX : Y ⊆ X) :
     M.IsRankCover ((· ∩ Y) '' T) Y k := by
-  rw [IsRankCover_iff_IsCover]
-  rw [IsRankCover_iff_IsCover] at hcov
-  apply hcov.mono_set hX
+  rw [IsRankCover_iff]
+  rw [IsRankCover_iff] at hcov
+  apply hcov.mono_subset hX
   intro F hF
   grw [eRk_subset_le M inter_subset_left, hF]
 
-lemma CoverNumberRank_le_sub (M : Matroid α) (k : ℕ∞) (hX : Y ⊆ X) :
-    Y.coverNumber (fun A ↦ M.eRk A ≤ k) ≤ X.coverNumber (fun A ↦ M.eRk A ≤ k) := by
-  obtain htop | ⟨T, hT, hTen ⟩ := X.exists_cover (fun A ↦ M.eRk A ≤ k)
-  · rw [htop]
-    exact OrderTop.le_top (Y.coverNumber fun A ↦ M.eRk A ≤ k)
-  rw [←IsRankCover_iff_IsCover] at hT
-  have := hT.mono_set hX
-  grw [(hT.mono_set hX ).coverNumber_le, ←hTen, encard_image_le (fun x ↦ x ∩ Y) T ]
-
-lemma IsRankCover.subset_union (hcov : M.IsRankCover T X k) (hne : X.Nonempty) (hX : X ⊆ M.E) :
+lemma IsRankCover.subset_union_closure (hcov : M.IsRankCover T X k) (hne : X.Nonempty) (hX : X ⊆ M.E) :
     X ∪ M.closure ∅ ⊆ ⋃ F ∈ T, M.closure F := by
   refine union_subset ?_ ?_
   · grw [←iUnion₂_mono (fun F hF ↦ subset_closure M F (hcov.subset_ground hF)),
@@ -446,7 +404,7 @@ lemma IsRankCover.subset_union (hcov : M.IsRankCover T X k) (hne : X.Nonempty) (
   grw [h1]
   exact subset_biUnion_of_mem hF'
 
-lemma IsRankCover.union_of_closure (hcov : M.IsRankCover T X k) (hD : D ⊆ M.loops)
+lemma IsRankCover.loops_union_of_closure (hcov : M.IsRankCover T X k) (hD : D ⊆ M.loops)
     (hne : X.Nonempty) (hX : X ⊆ M.E) :
     M.IsRankCover ( (· ∩ (X ∪ D)) '' (M.closure '' T)  ) (X ∪ D) k := by
   refine ⟨ ?_, ?_ ⟩
@@ -454,7 +412,7 @@ lemma IsRankCover.union_of_closure (hcov : M.IsRankCover T X k) (hD : D ⊆ M.lo
     rw [Eq.symm (iUnion₂_inter (fun i j ↦ M.closure i) (X ∪ D)) ]
     refine inter_eq_self_of_subset_right ?_
     grw [union_subset_union_right X hD ]
-    apply hcov.subset_union hne hX
+    apply hcov.subset_union_closure hne hX
   intro F hF
   simp only [mem_image, exists_exists_and_eq_and] at hF
   obtain ⟨F', hF', rfl ⟩ := hF
@@ -462,12 +420,11 @@ lemma IsRankCover.union_of_closure (hcov : M.IsRankCover T X k) (hD : D ⊆ M.lo
   simp only [eRk_closure_eq]
   exact hcov.pProp F' hF'
 
-
-lemma IsRankCover_isCover_flat_closure (hcov : M.IsRankCover T X k) (hX : M.IsFlat X) :
+lemma IsRankCover.isCover_flat_closure (hcov : M.IsRankCover T X k) (hX : M.IsFlat X) :
     M.IsRankCover (M.closure '' T) X k := by
-  rw [IsRankCover_iff_IsCover]
-  rw [IsRankCover_iff_IsCover]  at hcov
-  apply Set.IsCover.isCover_closure hcov (fun M F hF ↦ ?_) hX (hX.subset_ground)
+  rw [IsRankCover_iff]
+  rw [IsRankCover_iff]  at hcov
+  apply Set.IsCover.isCover_closure hcov (fun F hF ↦ ?_) hX (hX.subset_ground)
   rwa [(eRk_closure_eq M F) ]
 
 lemma IsRankCover.mono_k {k' : ℕ∞} (hcov : M.IsRankCover T X k) (hkk' : k ≤ k') :
@@ -475,34 +432,46 @@ lemma IsRankCover.mono_k {k' : ℕ∞} (hcov : M.IsRankCover T X k) (hkk' : k �
   refine ⟨ hcov.sUnion_eq, fun F hF ↦
     Std.IsPreorder.le_trans (M.eRk F) k k' (hcov.pProp F hF ) hkk' ⟩
 
-lemma IsRankCover.one_le (h : M.IsRankCover T X k) (hX : X.Nonempty) :
-    T.Nonempty := IsCover.one_le h hX
+lemma IsRankCover.nonempty_set (h : M.IsRankCover T X k) (hX : X.Nonempty) :
+    T.Nonempty := h.nonempty hX
 
 lemma IsRankCover_Zero (X : Set α) (hX : X ⊆ M.E := by aesop_mat) :
-    X.hasCover_with (fun A ↦ M.eRk A ≤ 0) ↔ X ⊆ M.loops := by
+    X.hasCover (fun A ↦ M.eRk A ≤ 0) ↔ X ⊆ M.loops := by
   refine ⟨ ?_, ?_ ⟩
   · intro h e he
     obtain ⟨ T', hT' ⟩ := h
     rw[←hT'.sUnion_eq ] at he
     obtain ⟨ Y, hYt, heY ⟩ := he
     apply isLoop_iff.mp
-    exact isLoop_iff.mp (((Matroid.eRk_eq_zero_iff ((IsRankCover_iff_IsCover.2 hT').subset_ground hYt  )).1
+    exact isLoop_iff.mp (((Matroid.eRk_eq_zero_iff ((IsRankCover_iff.2 hT').subset_ground hYt  )).1
       (nonpos_iff_eq_zero.mp (hT'.pProp Y hYt ))) heY)
   intro h
-  refine ⟨ (singleton '' X), IsCover_singleton_Prop ?_ ⟩
+  refine ⟨ (singleton '' X), isCover_image_singleton ?_ ⟩
   intro e he
   simp only [nonpos_iff_eq_zero]
   refine IsLoop.eRk_eq ?_
   exact isLoop_iff.mpr (h he)
 
-lemma IsRankCover_Zero_or' (X : Set α) (hne : X.Nonempty) (hX : X ⊆ M.E := by aesop_mat) :
-    ⊤ = X.coverNumber (fun A ↦ M.eRk A ≤ 0 ) ∨ ∃ F, M.IsRankCover ({M.closure F ∩ X}) X 0 := by
+lemma CoverNumberRank_subset_le (M : Matroid α) (k : ℕ∞) (hX : Y ⊆ X) :
+    M.coverNumberByRank Y k ≤ M.coverNumberByRank X k := by
+    --Y.coverNumber (fun A ↦ M.eRk A ≤ k) ≤ X.coverNumber (fun A ↦ M.eRk A ≤ k) := by
+  rw [coverNumberByRank_eq, coverNumberByRank_eq]
+  obtain htop | ⟨T, hT, hTen ⟩ := X.exists_cover (fun A ↦ M.eRk A ≤ k)
+  · rw [htop]
+    exact OrderTop.le_top (Y.coverNumber fun A ↦ M.eRk A ≤ k)
+  rw [←IsRankCover_iff] at hT
+  have := hT.mono_subset hX
+  grw [(hT.mono_subset hX ).coverNumber_le, ←hTen, encard_image_le (fun x ↦ x ∩ Y) T ]
+
+lemma IsRankCover_zero_or_exists' (X : Set α) (hne : X.Nonempty) (hX : X ⊆ M.E := by aesop_mat) :
+    ⊤ = M.coverNumberByRank X 0 ∨ ∃ F, M.IsRankCover ({M.closure F ∩ X}) X 0 := by
+  rw [coverNumberByRank_eq]
   obtain ht | ⟨T, hT, hT2 ⟩ := X.exists_cover (fun A ↦ M.eRk A ≤ 0 )
   · left
     rw [ht]
   right
-  rw [← IsRankCover_iff_IsCover ] at hT
-  obtain ⟨ F, hF ⟩:= hT.one_le hne
+  rw [← IsRankCover_iff ] at hT
+  obtain ⟨ F, hF ⟩:= hT.nonempty_set hne
   refine ⟨ F , ?_ ⟩
   have hsub := (IsRankCover_Zero X).1 ⟨T, hT⟩
   refine ⟨ ?_, ?_ ⟩
@@ -513,20 +482,20 @@ lemma IsRankCover_Zero_or' (X : Set α) (hne : X.Nonempty) (hX : X ⊆ M.E := by
   apply nonpos_iff_eq_zero.mp
   grw [eRk_subset_le M (inter_subset_right ), (eRk_eq_zero_iff hX).mpr hsub]
 
-lemma IsRankCover_Zero_or (X : Set α) (hne : X.Nonempty) (hX : X ⊆ M.E := by aesop_mat) :
-    ⊤ = X.coverNumber (fun A ↦ M.eRk A ≤ 0 ) ∨ X.coverNumber (fun A ↦ M.eRk A ≤ 0 ) = 1 := by
-  obtain htop | ⟨ F, hF ⟩ := IsRankCover_Zero_or' X hne
+lemma IsRankCover_zero_or_exists (X : Set α) (hne : X.Nonempty) (hX : X ⊆ M.E := by aesop_mat) :
+    ⊤ =  M.coverNumberByRank X 0 ∨ M.coverNumberByRank X 0 = 1 := by
+  rw [coverNumberByRank_eq]
+  obtain htop | ⟨ F, hF ⟩ := IsRankCover_zero_or_exists' X hne
   · left
     exact htop
   right
   have h1 := hF.coverNumber_le
   simp only [ encard_singleton] at h1
-  have h2 := coverNumber_positive hne (fun A ↦ M.eRk A ≤ 0 )
+  have h2 := one_le_coverNumber hne (fun A ↦ M.eRk A ≤ 0 )
   grind
 
-
-lemma IsRankCover_RankPos :
-    (M.E).hasCover_with (fun A ↦ M.eRk A ≤ 0) ↔ ¬ M.RankPos := by
+lemma IsRankCover_zero_iff_not_rankPos :
+    (M.E).hasCover (fun A ↦ M.eRk A ≤ 0) ↔ ¬ M.RankPos := by
   refine ⟨fun h ↦ (M.not_rankPos_iff.2 (Matroid.eq_loopyOn_iff_loops.mpr
     ⟨Eq.symm (Subset.antisymm ((IsRankCover_Zero M.E).1 h ) (loops_subset_ground M )),
     by simp only ⟩)) , fun h ↦ (IsRankCover_Zero M.E fun ⦃a⦄ a_1 ↦ a_1).mpr
@@ -539,7 +508,7 @@ lemma IsRankCover_RankPos :
 --   simp [IsRankCover_iff, eq_comm] at h
 --   exact Ne.elim (Set.nonempty_iff_empty_ne.1 hX ) (Eq.symm h)
 
-lemma IsRankCover.Nontrivial (hcov : M.IsRankCover T X k) (hk : k < M.eRk X ) :
+lemma IsRankCover.nontrivial (hcov : M.IsRankCover T X k) (hk : k < M.eRk X ) :
     T.Nontrivial := by
   by_contra hc
   have hXne : X.Nonempty := by
@@ -551,16 +520,16 @@ lemma IsRankCover.Nontrivial (hcov : M.IsRankCover T X k) (hk : k < M.eRk X ) :
     rw [eRk_empty M] at hg
     exact (lt_self_iff_false 0).mp hg
   simp only [not_nontrivial_iff] at hc
-  have h1 := hcov.one_le
+  have h1 := hcov.nonempty
   have h1 : T.encard = 1 := by grind
   obtain ⟨X', hX' ⟩ := Set.encard_eq_one.1 h1
-  have h2 := ((IsRankCover_iff_IsCover).1 hcov).sUnion_eq
+  have h2 := ((IsRankCover_iff).1 hcov).sUnion_eq
   rw [hX'] at h2
   simp only [sUnion_singleton] at h2
   have hXT : X' ∈ T := by
     rw[ hX' ]
     exact mem_singleton X'
-  have hf := ((IsRankCover_iff_IsCover).1 hcov).pProp X' hXT
+  have hf := ((IsRankCover_iff).1 hcov).pProp X' hXT
   rw[ h2] at hf
   grind
 
@@ -578,7 +547,8 @@ lemma setOf_point_IsRankCover (M : Matroid α) (X : Set α) [(M ↾ X).RankPos] 
   simp only [restrict_ground_eq] at hgs
   grw [← inter_eq_left.2 (LE.le.subset hgs), ←restrict_eRk_eq', hF.eRk ]
 
-lemma setOf_point_IsCover [hM : (M ↾ X).Loopless] : M.IsRankCover {P | (M ↾ X).IsPoint P} X 1 := by
+lemma setOf_point_IsRankCover' [hM : (M ↾ X).Loopless] :
+    M.IsRankCover {P | (M ↾ X).IsPoint P} X 1 := by
   obtain ⟨E, hX⟩ | h := (M ↾ X).eq_loopyOn_or_rankPos'
   · rw [hX]
     rw [hX] at hM
@@ -596,16 +566,10 @@ lemma IsRankCover_ground (M : Matroid α) : M.IsRankCover ({X}) X (M.eRk X) := b
   simp only [mem_singleton_iff] at hF
   rw [hF]
 
-lemma IsRankCover.nonempty (h : M.IsRankCover T X k) (hX : X.Nonempty) : T.Nonempty := by
-  rw [nonempty_iff_empty_ne]
-  rintro rfl
-  simp [IsRankCover_iff, eq_comm] at h
-  exact Ne.elim (Set.nonempty_iff_empty_ne.1 hX ) (Eq.symm h)
-
-lemma RankPropCover_exists (M : Matroid α) (hk : 1 ≤ k) (hX : X ⊆ M.E) :
-    X.hasCover_with (fun A ↦ M.eRk A ≤ k) := by
+lemma coverNumberByRank_exists (M : Matroid α) (hk : 1 ≤ k) (hX : X ⊆ M.E) :
+    X.hasCover (fun A ↦ M.eRk A ≤ k) := by
   by_cases hRP : (M ↾ X).RankPos
-  · refine ⟨{P | (M ↾ X).IsPoint P}, IsRankCover_iff_IsCover.1
+  · refine ⟨{P | (M ↾ X).IsPoint P}, IsRankCover_iff.1
       ((M.setOf_point_IsRankCover X ).mono_k hk) ⟩
   have hXl : X ⊆ M.loops := by
     rw [not_rankPos_iff, restrict_ground_eq] at hRP
@@ -613,18 +577,30 @@ lemma RankPropCover_exists (M : Matroid α) (hk : 1 ≤ k) (hX : X ⊆ M.E) :
     rw [Eq.symm (eRank_restrict M X), hRP]
     exact eRank_loopyOn X
   obtain ⟨ T, hT ⟩ := (IsRankCover_Zero X).2 hXl
-  refine ⟨ T, IsRankCover_iff_IsCover.1 (IsRankCover.mono_k hT (ENat.zero_le))⟩
+  refine ⟨ T, IsRankCover_iff.1 (IsRankCover.mono_k hT (ENat.zero_le))⟩
 
-lemma RankPropCover_exists_min_cover (M : Matroid α) (hk : 1 ≤ k) (hX : X ⊆ M.E) :
-    ∃ T, M.IsRankCover T X k ∧ T.encard = X.coverNumber (fun A ↦ M.eRk A ≤ k) := by
-  simp only [IsRankCover_iff_IsCover]
-  exact exists_min_cover (RankPropCover_exists M hk hX)
+lemma coverNumberByRank_exists_cover (M : Matroid α) (X : Set α) (k : ℕ∞) :
+    M.coverNumberByRank X k = ⊤ ∨ ∃ T, M.IsRankCover T X k ∧ T.encard = M.coverNumberByRank X k
+    := by
+  exact exists_cover X (fun A ↦ M.eRk A ≤ k)
 
-lemma RankCoverNumber_eq :
-    X.coverNumber (fun A ↦ M.eRk A ≤ a ) = X.coverNumber (fun A ↦ (M ↾ X).eRk A ≤ a ) := by
+lemma RankPropCover_exists_encard_eq (M : Matroid α) (hk : 1 ≤ k) (hX : X ⊆ M.E) :
+    ∃ T, M.IsRankCover T X k ∧ T.encard = M.coverNumberByRank X k := by
+  simp only [IsRankCover_iff]
+  exact exists_encard_eq_coverNumber (coverNumberByRank_exists M hk hX)
+
+lemma coverNumberByRank_restriction_eq :
+    M.coverNumberByRank X a = (M ↾ X).coverNumberByRank X a  := by
   refine coverNumber_congr (fun A ↦ M.eRk A ≤ a) (fun A ↦ (M ↾ X).eRk A ≤ a) ?_
   intro Y hY
   simp only [restrict_eRk_eq M hY]
+
+lemma IsRankCover.coverNumberByRank_le {T : Set (Set α)} (h : M.IsRankCover T X k ) :
+    M.coverNumberByRank X k ≤ T.encard := by
+  rw [coverNumberByRank_eq]
+  rw [IsRankCover_iff] at h
+  exact h.coverNumber_le
+
 
 lemma IsRankCover.delete (hT : M.IsRankCover T X k) (D : Set α) :
     M.IsRankCover ((fun s ↦ s \ D) '' T) (X \ D) k := by
@@ -645,56 +621,62 @@ lemma IsRankCover.delete (hT : M.IsRankCover T X k) (D : Set α) :
   grw [eRk_subset_le M (diff_subset)]
   exact hT.pProp F' hF'
 
-lemma IsRankcoverNumber_eRk (hX : X.Nonempty) :
-    X.coverNumber (fun A ↦ M.eRk A ≤ (M.eRk X)) = 1 := by
+lemma coverNumberByRank_eRk (hX : X.Nonempty) :
+    M.coverNumberByRank X (M.eRk X) = 1 := by
   have h2 : 1 ≤ X.coverNumber (fun A ↦ M.eRk A ≤ (M.eRk X)) :=
-    coverNumber_positive hX (fun A ↦ M.eRk A ≤ (M.eRk X))
+    one_le_coverNumber hX (fun A ↦ M.eRk A ≤ (M.eRk X))
   refine h2.antisymm' ?_
   simpa using (IsRankCover_ground M).coverNumber_le
 
-lemma IsRankcoverNumber_delete_loop (hD : D ⊆ M.loops ) (hne : (X \ D).Nonempty )
+lemma coverNumberByRank_delete_loop (hD : D ⊆ M.loops ) (hne : (X \ D).Nonempty )
     (hX : X ⊆ M.E) :
-    X.coverNumber (fun A ↦ M.eRk A ≤ k) = (X \ D).coverNumber (fun A ↦ M.eRk A ≤ k) := by
-  have h1 := CoverNumberRank_le_sub M k (diff_subset (s := X) (t := D))
+    M.coverNumberByRank X k = M.coverNumberByRank (X \ D) k := by
+  have h1 := CoverNumberRank_subset_le M k (diff_subset (s := X) (t := D))
   have hh : X \ D ⊆ M.E := by
     simp only [diff_subset_iff, subset_union_of_subset_right hX D ]
   obtain ht | ⟨T', hT', hT'en ⟩ := (X \ D).exists_cover (fun A ↦ M.eRk A ≤ k)
-  · rw [ht] at h1
+  · rw [←coverNumberByRank_eq] at ht
+    rw [ht] at h1
     rw [ht]
     grind
-  rw [←IsRankCover_iff_IsCover] at hT'
-  have hcov := hT'.union_of_closure (D := D ∩ X)
+  rw [←IsRankCover_iff] at hT'
+  have hcov := hT'.loops_union_of_closure (D := D ∩ X)
     (LE.le.subset fun ⦃a⦄ a_1 ↦ hD (inter_subset_left a_1) ) hne hh
-  have h2 := hcov.coverNumber_le
+  have h2 := hcov.coverNumberByRank_le
   have : (X \ D) ∪ (D ∩ X) = X := by grind
   grw [this, encard_image_le (fun x ↦ x ∩ X) (M.closure '' T'),
     encard_image_le M.closure T', hT'en] at h2
+  rw [←coverNumberByRank_eq] at h2
   grind
 
---Ask
-lemma IsRankcoverNumber_contract_one {a : ℕ∞} (hel : M.IsNonloop e) (heX : e ∈ X)
+lemma coverNumberByRank_contract_one {a : ℕ∞} (hel : M.IsNonloop e) (heX : e ∈ X)
     (hne : (X \ {e}).Nonempty) :
-    X.coverNumber (fun A ↦ M.eRk A ≤ (a + 1)) ≤ (X \ {e}).coverNumber (fun A ↦ (M ／ {e}).eRk A ≤ a)
+    M.coverNumberByRank X (a + 1) ≤ (M ／ {e}).coverNumberByRank (X \ {e}) a
+    -- (X \ {e}).coverNumber (fun A ↦ (M ／ {e}).eRk A ≤ a)
+    -- X.coverNumber (fun A ↦ M.eRk A ≤ (a + 1)) ≤ (X \ {e}).coverNumber (fun A ↦ (M ／ {e}).eRk A ≤ a)
     := by
-  obtain ht | ⟨T, hT, hT' ⟩ := (X \ {e}).exists_cover (fun A ↦ (M ／ {e}).eRk A ≤ a)
+  obtain ht | ⟨T, hT, hT' ⟩ := coverNumberByRank_exists_cover (M ／ {e}) (X \ {e}) a
+  -- obtain ht | ⟨T, hT, hT' ⟩ := (X \ {e}).exists_cover (fun A ↦ (M ／ {e}).eRk A ≤ a)
   · rw [ht]
     exact OrderTop.le_top (X.coverNumber fun A ↦ M.eRk A ≤ a + 1)
   have hcov : ((fun x ↦ x ∪ {e}) '' T).IsCover X fun A ↦ M.eRk A ≤ (a + 1) := by
     have hrw : X = X \ {e} ∪ {e} := by grind
     nth_rw 1 [hrw]
-    apply hT.contract hne (P' := (fun A ↦ M.eRk A ≤ a + 1)) (P := (fun A ↦ (M ／ {e}).eRk A ≤ a)) (X := {e})
+    apply hT.image_union hne (P' := (fun A ↦ M.eRk A ≤ a + 1))
+      (P := (fun A ↦ (M ／ {e}).eRk A ≤ a)) (X := {e})
     intro F hF
     rw [←eRelRk_eq_eRk_contract M {e} F] at hF
     grw [ ←eRelRk_add_eRk_eq M {e} F, IsNonloop.eRk_eq hel]
     simp only [ne_eq, ENat.one_ne_top, not_false_eq_true, add_le_add_iff_left_of_ne_top]
     exact hF
-  grw [←hT', hcov.coverNumber_le]
+  rw [←IsRankCover_iff] at hcov
+  grw [←hT', hcov.coverNumberByRank_le ]
   simp only [union_singleton, ge_iff_le]
   exact encard_image_le (fun a ↦ insert e a) T
 
 
-lemma IsRankcoverNumber_contract_one' {a : ℕ∞} (hel : M.IsNonloop e) :
-    X.coverNumber (fun A ↦ M.eRk A ≤ (a + 1)) ≤ X.coverNumber (fun A ↦ (M ／ {e}).eRk A ≤ a)
+lemma coverNumberByRank_contract_one' {a : ℕ∞} (hel : M.IsNonloop e) :
+    M.coverNumberByRank X (a + 1) ≤ (M ／ {e}).coverNumberByRank X a
     := by
   refine coverNumber_le_coverNumber (fun A ↦ (M ／ {e}).eRk A ≤ a) (fun A ↦ M.eRk A ≤ a + 1) X ?_
   intro Y hY
@@ -783,8 +765,7 @@ lemma base_isCover {a : ℕ} (hr : M.eRank ≤ a + 1) (ha : 1 ≤ a) (hXfin : X.
 
 lemma baseCase {a b : ℕ} (ha : 1 ≤ a) (hM : NoUniformMinor M (a + 1) (b + 1))
     (hr : M.eRank = a + 1) :
-    (M.E).coverNumber (fun A ↦ M.eRk A ≤ a ) ≤ Nat.choose b a := by
-    --M.coverNumber (fun M X ↦ M.eRk X ≤ a) ≤ Nat.choose b a := by
+    M.coverNumberByRank M.E a ≤ Nat.choose b a := by
   have : M.RankFinite := M.eRank_ne_top_iff.mp (ENat.ne_top_iff_exists.2
       (Exists.intro ((fun x1 x2 ↦ x1 + x2) a 1) (hr.symm)))
   by_contra! hcon
@@ -799,16 +780,12 @@ lemma baseCase {a b : ℕ} (ha : 1 ≤ a) (hM : NoUniformMinor M (a + 1) (b + 1)
     intro X hX
     by_contra hc
     simp only [not_lt] at hc
-    --have : X ⊆ M.E := by exact hX.1
     have h2 : ((unifOn (M ↾ X).E (a + 1)).NoUniformMinor (a + 1) (b + 1)) := by
       rw[←hX.2.eq_unifOn ]
       exact hM.minor (IsRestriction.isMinor (restrict_isRestriction M X) )
     have h3 := unifOn_noUniformMinor_iff.1 h2
     grw [← restrict_ground_eq (M := M) (R := X)] at hc
     grind
-    --simp only [mem_setOf_eq] at hX
-    -- exact hc.not_gt <| hM.lt_of_isoMinor (N := M ↾ X) (b' := X.encard)
-    --   (restrict_isRestriction _ _ hX.1).isMinor.isoMinor sorry
   have hcard : (encard '' Unif).Finite := by
     refine ENat.finite_of_sSup_lt_top ?_
     refine lt_of_le_of_lt ?_ <| WithTop.natCast_lt_top (b + 1)
@@ -819,26 +796,26 @@ lemma baseCase {a b : ℕ} (ha : 1 ≤ a) (hM : NoUniformMinor M (a + 1) (b + 1)
   obtain ⟨X, hX⟩ := Finite.exists_maximalFor' encard _ hcard hne
   have hXb : X.encard < b + 1 := hYbound X hX.prop
   set Subsets : Set (Set α) := { Y | Y ⊆ X ∧ Y.encard = a} with h_sub
-  --(Set.encard_le_coe_iff.1 (ENat.lt_coe_add_one_iff.mp hXb )).1
   have hiC := base_isCover (Std.le_of_eq hr ) ha
       ((Set.encard_le_coe_iff.1 (ENat.lt_coe_add_one_iff.mp hXb )).1) hX
-  --have hiC : M.IsCover (fun M X ↦ M.eRk X ≤ a) (M.closure '' Subsets) := by base_isCover
   obtain ⟨x, hx ⟩ := ENat.ne_top_iff_exists.1 (LT.lt.ne_top hXb )
   rw[←hx] at hXb
-  grw [hiC.coverNumber_le, Set.encard_image_le, (set_to_binom_number) X hx.symm,
+  grw [hiC.coverNumberByRank_le, Set.encard_image_le, (set_to_binom_number) X hx.symm,
     (Nat.choose_le_choose a (Nat.le_of_lt_succ (ENat.coe_lt_coe.mp hXb )))] at hcon
   simp only [lt_self_iff_false] at hcon
 
-lemma coverNumber_rank_Frombase {a b : ℕ} (ha : 1 ≤ a)
+lemma coverNumberByRank_from_base {a b : ℕ} (ha : 1 ≤ a)
     (hM : NoUniformMinor M ( a + 1 ) (b + 1)) :
-    M.E.coverNumber (fun A ↦ M.eRk A ≤ a) ≤
-    (Nat.choose b a) * (M.E).coverNumber (fun A ↦ M.eRk A ≤ a + 1) := by
+    M.coverNumberByRank M.E a ≤
+    (Nat.choose b a) * coverNumberByRank M M.E (a + 1) := by
+    -- M.E.coverNumber (fun A ↦ M.eRk A ≤ a) ≤
+    -- (Nat.choose b a) * (M.E).coverNumber (fun A ↦ M.eRk A ≤ a + 1) := by
   sorry
 
-lemma coverNumber_Bound {M : Matroid α} [M.RankPos] {a b : ℕ} {n : ℕ∞} (ha : a ≠ 0) (hb : a ≤ b)
+lemma coverNumberByRank_le_binomial {M : Matroid α} [M.RankPos] {a b : ℕ} {n : ℕ∞} (ha : a ≠ 0)
+    (hb : a ≤ b)
     (hM : NoUniformMinor M (a + 1) (b + 1)) (hn : M.eRank = a + n) :
-    M.E.coverNumber (fun A ↦ M.eRk A ≤ a ) ≤ (Nat.choose b a)^n := by
-    --M.coverNumber (fun M X ↦ M.eRk X ≤ a) ≤ (Nat.choose b a)^(M.eRank - a) := by
+    M.coverNumberByRank M.E a ≤ (Nat.choose b a)^n := by
   obtain htop | hfin := eq_or_ne M.eRank ⊤
   · grw [htop] at hn
     have hrw : n = ⊤ := by
@@ -858,30 +835,27 @@ lemma coverNumber_Bound {M : Matroid α} [M.RankPos] {a b : ℕ} {n : ℕ∞} (h
   have hRP : ( M ／ {e}).RankPos := by sorry --I think here you need n ≠ 0
   have hM' : NoUniformMinor ( M ／ {e}) ( a + 1 ) (b + 1) := by sorry
   have hn' : (M ／ {e}).eRank = a + (n - 1) := by sorry
-  have ih := coverNumber_Bound (M := M ／ {e}) (a := a) (b := b) ha hb hM' (n := n - 1)
+  have ih := coverNumberByRank_le_binomial (M := M ／ {e}) (a := a) (b := b) ha hb hM' (n := n - 1)
   sorry
 termination_by M.eRank
 
-lemma coverNumber_Bound_subset {M : Matroid α} [(M ↾ Y).RankPos] {a b : ℕ} {n : ℕ∞} (ha : a ≠ 0)
+lemma coverNumberByRank_le_binomial_subset {M : Matroid α} [(M ↾ Y).RankPos] {a b : ℕ} {n : ℕ∞} (ha : a ≠ 0)
     (hb : a ≤ b)
     (hM : (M ↾ Y).NoUniformMinor (a + 1) (b + 1)) (hn : M.eRk Y = a + n) :
-    Y.coverNumber (fun A ↦ M.eRk A ≤ a ) ≤ (Nat.choose b a)^n := by
-  rw [RankCoverNumber_eq ]
-  nth_rw 1 [←restrict_ground_eq (M := M) (R := Y)]
-  exact coverNumber_Bound ha hb hM hn
+     M.coverNumberByRank Y a ≤ (Nat.choose b a)^n := by
+  rw [coverNumberByRank_restriction_eq ]
+  exact coverNumberByRank_le_binomial ha hb hM hn
 
-lemma coverNumber_Bound_contract {M : Matroid α} {C : Set α} {a b : ℕ} (ha : a ≠ 0) (hb : a ≤ b)
+lemma coverNumberByRank_le_binomial_contract {M : Matroid α} {C : Set α} {a b : ℕ} (ha : a ≠ 0) (hb : a ≤ b)
     (hM : NoUniformMinor M (a + 1) (b + 1)) (hC : C ⊂ M.E)  :
-    (M.E).coverNumber (fun A ↦ M.eRk A ≤ a) ≤
-    (Nat.choose b a)^(M.eRk C) * (M ／ C).E.coverNumber (fun A ↦ (M ／ C).eRk A ≤ a) := by
-    --M.coverNumber (fun M X ↦ M.eRk X ≤ a) ≤
-    --(Nat.choose b a)^(M.eRk C) * (M ／ C).coverNumber (fun M X ↦ M.eRk X ≤ a) := by
+    M.coverNumberByRank M.E a ≤
+    (Nat.choose b a)^(M.eRk C) * (M ／ C).coverNumberByRank (M ／ C).E a := by
   obtain htop | hlt := eq_or_ne (M.eRk C) ⊤
   · grw [htop, ENat.epow_top, ENat.top_mul, ← le_top ]
     · have heN : (M／ C).Nonempty := by
         rw[←(M／ C).ground_nonempty_iff, contract_ground]
         exact (Set.nonempty_of_ssubset (by grind ) )
-      exact ENat.one_le_iff_ne_zero.mp (coverNumber_positive
+      exact ENat.one_le_iff_ne_zero.mp (one_le_coverNumber
         ((ground_nonempty_iff (M ／ C)).mpr heN) (fun A ↦ (M ／ C).eRk A ≤ a ) )
     obtain rfl | hlt := hb.eq_or_lt
     · simp [noUniformMinor_self_iff] at hM
@@ -893,10 +867,9 @@ lemma coverNumber_Bound_contract {M : Matroid α} {C : Set α} {a b : ℕ} (ha :
   obtain h0 | hn := eq_or_ne (M.eRk C) 0
   · rw [h0]
     simp only [ENat.epow_zero, contract_ground, one_mul]
-    rw [IsRankcoverNumber_delete_loop ((eRk_eq_zero_iff (subset_of_ssubset hC )).mp h0 )
+    rw [coverNumberByRank_delete_loop ((eRk_eq_zero_iff (subset_of_ssubset hC )).mp h0 )
       (nonempty_of_ssubset hC ) (by simp) ]
-    suffices h : ((M.E \ C).coverNumber fun A ↦ M.eRk A ≤ ↑a) =
-      (M.E \ C).coverNumber fun A ↦ (M ／ C).eRk A ≤ ↑a
+    suffices h : M.coverNumberByRank (M.E \ C) a = (M ／ C).coverNumberByRank (M.E \ C) ↑a
     · rw [h]
     refine coverNumber_congr (fun A ↦ M.eRk A ≤ ↑a) (fun A ↦ (M ／ C).eRk A ≤ ↑a) ?_
     intro Y hY
@@ -906,11 +879,8 @@ lemma coverNumber_Bound_contract {M : Matroid α} {C : Set α} {a b : ℕ} (ha :
     simp only [M.delete_eRk_eq h ]
   have hresP : (M ↾ C).RankPos := (eRank_ne_zero_iff (M ↾ C)).mp <|
     by simp [eRank_restrict, ne_eq, hn]
-    -- (eRank_ne_zero_iff (M ↾ C)).mp <| by simp [eRank_restrict, ne_eq, ← hn]
   obtain ⟨e, heC⟩ : ∃ e, (M ↾ C).IsNonloop e := exists_isNonloop (M ↾ C)
   rw [restrict_isNonloop_iff] at heC
-  -- have hrelrk := IsNonloop.eRelRk_add_one_eq heC.1 (C \ {e})
-  -- simp only [insert_diff_singleton, insert_eq_of_mem heC.2] at hrelrk
   have h' : (M ／ {e}).eRk (C \ {e}) < M.eRk C := by
     have hrelrk := IsNonloop.eRelRk_add_one_eq heC.1 (C \ {e})
     simp only [insert_diff_singleton, insert_eq_of_mem heC.2] at hrelrk
@@ -931,11 +901,11 @@ lemma coverNumber_Bound_contract {M : Matroid α} {C : Set α} {a b : ℕ} (ha :
   have heN : (M／ {e}).Nonempty := by
     rw[←(M／ {e}).ground_nonempty_iff, contract_ground]
     exact (Set.nonempty_of_ssubset (by grind ) )
-  have ih := coverNumber_Bound_contract (M := M ／ {e}) (C := C \ {e}) (a := a) (b := b) ha
+  have ih := coverNumberByRank_le_binomial_contract (M := M ／ {e}) (C := C \ {e}) (a := a) (b := b) ha
     hb (hM.minor (contract_isMinor M {e} )) hsub1
   nth_rw 1 [contract_ground M {e} ] at ih
-  grw [coverNumber_rank_Frombase (Nat.one_le_iff_ne_zero.mpr ha) hM,
-    IsRankcoverNumber_contract_one heC.1 (mem_of_subset_of_mem (subset_of_ssubset hC ) (heC.2 ))
+  grw [coverNumberByRank_from_base (Nat.one_le_iff_ne_zero.mpr ha) hM,
+    coverNumberByRank_contract_one heC.1 (mem_of_subset_of_mem (subset_of_ssubset hC ) (heC.2 ))
     (nonempty_of_ssubset' hsub1 ), ih ]
   simp only [contract_contract, union_diff_self, singleton_union, ge_iff_le, insert_eq_of_mem heC.2,
     ←mul_assoc]
@@ -949,6 +919,7 @@ termination_by M.eRk C
 end Rank
 
 section NonSpanning
+
 
 /-- Docstring here -/
 def NonSpanningCover (M : Matroid α) (T : Set (Set α)) (X : Set α) :=
@@ -967,10 +938,10 @@ lemma nonSpanningCover_iff_restriction :
   rw [nonSpanningCover_iff, restrict_ground_eq, restrict_idem] at h
   exact nonSpanningCover_iff.mpr h
 
-lemma NonSpanning_le_RankCover {n : ℕ} (hr : M.eRk X = n + 1) :
-    X.coverNumber (M ↾ X).Nonspanning ≤ X.coverNumber (fun A ↦ M.eRk A ≤ n ) := by
+lemma nonSpanning_le_coverNumberByRank {n : ℕ} (hr : M.eRk X = n + 1) :
+    X.coverNumber (M ↾ X).Nonspanning ≤ M.coverNumberByRank X n := by
   obtain ht | ⟨T, hT, hT' ⟩ := X.exists_cover (fun A ↦ M.eRk A ≤ n)
-  · rw [ht]
+  · rw [coverNumberByRank ,ht]
     exact OrderTop.le_top (X.coverNumber (M ↾ X).Nonspanning)
   have hcov :  T.IsCover X (M ↾ X).Nonspanning := by
     refine ⟨hT.sUnion_eq, ?_⟩
@@ -980,28 +951,9 @@ lemma NonSpanning_le_RankCover {n : ℕ} (hr : M.eRk X = n + 1) :
     simp only [restrict_eRk_eq M (hT.subset hF), eRank_restrict, ne_eq, hr]
     enat_to_nat! <;>
     grind
-  grw [←hT', hcov.coverNumber_le]
+  grw [coverNumberByRank, ←hT', hcov.coverNumber_le]
 
-
--- lemma NonSpanning_to_RankCover (h : M.IsRkFinite X) (h0 : M.eRk X ≠ 0) :
---     NonSpanningCover M T X ↔ M.IsRankCover T X (M.eRk X - 1) := by sorry
-    --M.IsCover Matroid.Nonspanning T ↔ M.IsRankCover (M.eRank - 1) T := by
-  -- rw [NonSpanningCover, IsRankCover, iff_comm, isCover_iff_isCover_subset]
-  -- convert Iff.rfl with A
-  -- have : (M ↾ X).RankFinite := sorry
-  -- by_cases hAX : A ⊆ X
-  -- rw [nonspanning_iff_eRk_lt]
-
-  -- refine ⟨?_, ?_ ⟩
-  -- · intro h
-  --   refine ⟨ h.sUnion_eq, ?_ ⟩
-  --   intro F hF
-  --   by_contra hc
-  --   simp only [not_le] at hc
-  --   sorry
-  -- sorry
-
-lemma NonSpaning_le_two (hX : X.Nonempty) (hle : M.eRk X ≤ 1) :
+lemma top_le_nonSpanning (hX : X.Nonempty) (hle : M.eRk X ≤ 1) :
     ⊤ ≤ X.coverNumber (M ↾ X).Nonspanning := by
   --rw [NonSpanningCover_iff]
   obtain hT | ⟨T, hT1, hT2 ⟩  := X.exists_cover (M ↾ X).Nonspanning
@@ -1035,7 +987,7 @@ lemma NonSpaning_le_two (hX : X.Nonempty) (hle : M.eRk X ≤ 1) :
     (hT1.subset hT') ).2 h2)) hT2
 
 
-lemma Non_spanning_singleton (he : e ∈ M.E) (hM : 2 ≤ M.eRank) : M.Nonspanning {e} := by
+lemma nonSpanning_singleton (he : e ∈ M.E) (hM : 2 ≤ M.eRank) : M.Nonspanning {e} := by
     by_contra hc
     have h1 : M.eRank ≤ 1 := by
       rw [not_nonspanning_iff] at hc
@@ -1044,20 +996,19 @@ lemma Non_spanning_singleton (he : e ∈ M.E) (hM : 2 ≤ M.eRank) : M.Nonspanni
     grw [←hM] at h1
     simp only [ENat.not_ofNat_le_one] at h1
 
-lemma IsCover_singleton_NonSpanning (hM : 2 ≤ M.eRk X) :
+lemma isCover_singleton_nonSpanning (hM : 2 ≤ M.eRk X) :
     NonSpanningCover M (singleton '' X) X := by
     --M.IsCover (Matroid.Nonspanning) (singleton '' M.E) := by
-  exact IsCover_singleton_Prop (fun e he ↦ Non_spanning_singleton he hM)
+  exact isCover_image_singleton (fun e he ↦ nonSpanning_singleton he hM)
 
-lemma IsCover_singleton_le_NonSpanning (hM : 2 ≤ M.eRk X) :
+lemma nonSpanningNumber_le (hM : 2 ≤ M.eRk X) :
     X.coverNumber ((M ↾ X).Nonspanning) ≤ X.encard := by
-  exact IsCover_singleton_le (fun e he ↦ Non_spanning_singleton he hM)
+  exact isCover_singleton_le (fun e he ↦ nonSpanning_singleton he hM)
 
-lemma NonSpaning_cover_exists (hM : 2 ≤ M.eRk X) : X.hasCover_with ((M ↾ X).Nonspanning) := by
-  refine ⟨(singleton '' X), IsCover_singleton_NonSpanning hM ⟩
+lemma nonSpanning_hasCover (hM : 2 ≤ M.eRk X) : X.hasCover ((M ↾ X).Nonspanning) := by
+  refine ⟨(singleton '' X), isCover_singleton_nonSpanning hM ⟩
 
-lemma IsNonSpaningCover_contract (h : NonSpanningCover (M ／ C) T (M.E \ C))
-    --(h : (M ／ X).IsCover (Matroid.Nonspanning) T)
+lemma nonSpanning_image_union (h : NonSpanningCover (M ／ C) T (M.E \ C))
     (hX : C ⊆ M.E) (hXN : (M ／ C).Nonempty) :
     NonSpanningCover M ((· ∪ C) '' T) M.E := by
   rw [nonSpanningCover_iff] at h
@@ -1065,7 +1016,7 @@ lemma IsNonSpaningCover_contract (h : NonSpanningCover (M ／ C) T (M.E \ C))
   have : (M.E \ C ∪ C) = M.E := by grind
   nth_rw 1 [← this]
   rw [←Matroid.ground_nonempty_iff, contract_ground] at hXN
-  apply h.contract (X := C) hXN
+  apply h.image_union (X := C) hXN
   intro F hF
   have h3 :  (M ／ C ↾ M.E \ C) = M ／ C := by
     simp only [restrict_eq_self_iff, contract_ground]
@@ -1082,7 +1033,7 @@ lemma IsNonSpaningCover_contract (h : NonSpanningCover (M ／ C) T (M.E \ C))
   rw [←not_spanning_iff (hF.subset_ground)] at hF
   exact Ne.elim (fun a ↦ hF hcc) h3
 
-lemma IsNonSpaningCover_contract_subset (h : NonSpanningCover (M ／ C) T (Y \ C) )
+lemma nonSpanning_image_union_subset (h : NonSpanningCover (M ／ C) T (Y \ C) )
     (hX : C ⊆ Y) (hY : (Y \ C).Nonempty) :
     NonSpanningCover M ((· ∪ C) '' T) Y := by
   have h1 : NonSpanningCover ( (M ↾ Y) ／ C) T (((M ↾ Y)).E \ C) := by
@@ -1092,39 +1043,10 @@ lemma IsNonSpaningCover_contract_subset (h : NonSpanningCover (M ／ C) T (Y \ C
     rw [restrict_contract_eq_contract_restrict M hX, restrict_idem]
     exact h.pProp F hF
   rw [nonSpanningCover_iff_restriction ]
-  exact IsNonSpaningCover_contract h1 (IsLoopEquiv.subset_ground rfl hX )
+  exact nonSpanning_image_union h1 (IsLoopEquiv.subset_ground rfl hX )
     ((ground_nonempty_iff ((M ↾ Y) ／ C)).mp hY )
 
--- lemma IsNonSpaningCover_contract_subset' (h : NonSpanningCover (M ／ C) T Y )
---     (hY : Y.Nonempty) :
---     NonSpanningCover M ((· ∪ C) '' T) (Y ∪ C) := by
---   rw [NonSpanningCover_iff] at h
---   rw [NonSpanningCover_iff]
---   apply h.contract (X := C) hY
---   intro F hF
---   by_contra hc
---   have hcc : (M ／ C ↾ Y).Spanning F := by
---     have hr : F ∪ C ⊆ (M ↾ (Y ∪ C)).E := by
---       simp only [restrict_ground_eq, union_subset_iff, subset_union_right, and_true]
---       exact subset_union_of_subset_left hF.subset_ground C
---     rw [not_nonspanning_iff hr] at hc
---     -- have hhY : Y ⊆ (M ／ C).E := by
---     --   simp only [contract_ground]
---     --   sorry
---     -- apply (restrict_spanning_iff (hF.subset_ground) ).2
---     refine ⟨?_, ?_ ⟩
---     sorry
---     --simp only [restrict_closure_eq, contract_closure_eq, contract_ground, restrict_ground_eq]
-
---     --simp only [union_diff_right] at h1
-
---     sorry
---   rw [←not_nonspanning_iff (hF.subset_ground)] at hcc
---   exact (iff_false_intro hcc).mp hF
-
-  --rw [←Matroid.ground_nonempty_iff, contract_ground] at hY
-
-lemma NonSpanningNumber_contract (hX : C ⊆ M.E) (hXN : (M ／ C).Nonempty) :
+lemma nonSpanningNumber_le_contract (hX : C ⊆ M.E) (hXN : (M ／ C).Nonempty) :
     M.E.coverNumber M.Nonspanning ≤ (M.E \ C).coverNumber (M ／ C).Nonspanning := by
   obtain hT | ⟨T, hT, hTe ⟩ := (M.E \ C).exists_cover (M ／ C).Nonspanning
   · rw [hT]
@@ -1132,13 +1054,13 @@ lemma NonSpanningNumber_contract (hX : C ⊆ M.E) (hXN : (M ／ C).Nonempty) :
   rw [← hTe]
   rw [←(restrict_ground_eq_self (M ／ C)), contract_ground M C,
     ←nonSpanningCover_iff (T := T ) (X := M.E \ C) (M := M ／ C)] at hT
-  have hrw2 := ((IsNonSpaningCover_contract hT hX hXN).coverNumber_le)
+  have hrw2 := ((nonSpanning_image_union hT hX hXN).coverNumber_le)
   simp only [restrict_ground_eq_self] at hrw2
   exact
     Std.IsPreorder.le_trans (M.E.coverNumber M.Nonspanning) ((fun x ↦ x ∪ C) '' T).encard T.encard
       hrw2 (encard_image_le (fun x ↦ x ∪ C) T )
 
-lemma NonSpanningNumber_contract_subset (hX : C ⊆ Y) (hYne : (Y \ C).Nonempty) :
+lemma nonSpanningNumber_le_contract_subset (hX : C ⊆ Y) (hYne : (Y \ C).Nonempty) :
     Y.coverNumber (M ↾ Y).Nonspanning ≤ (Y \ C).coverNumber ((M ／ C) ↾ (Y \ C)).Nonspanning := by
   obtain hT | ⟨T, hT, hTe ⟩ := (Y \ C).exists_cover ((M ／ C) ↾ (Y \ C)).Nonspanning
   · rw [hT]
@@ -1147,23 +1069,10 @@ lemma NonSpanningNumber_contract_subset (hX : C ⊆ Y) (hYne : (Y \ C).Nonempty)
   rw [←nonSpanningCover_iff (T := T ) (X := Y \ C) (M := M ／ C)] at hT
   exact
     Std.IsPreorder.le_trans (Y.coverNumber (M ↾ Y).Nonspanning) ((fun x ↦ x ∪ C) '' T).encard T.encard
-      ((IsNonSpaningCover_contract_subset hT hX hYne).coverNumber_le)
+      ((nonSpanning_image_union_subset hT hX hYne).coverNumber_le)
       (encard_image_le (fun x ↦ x ∪ C) T )
 
--- lemma NonSpanningNumber_contract_subset' (hYne : (Y \ C).Nonempty) :
---     Y.coverNumber (M ↾ Y).Nonspanning ≤ Y.coverNumber ((M ／ C) ↾ Y).Nonspanning := by
---   obtain hT | ⟨T, hT, hTe ⟩ := Y.exists_cover ((M ／ C) ↾ Y).Nonspanning
---   · rw [hT]
---     exact OrderTop.le_top (Y.coverNumber (M ↾ Y).Nonspanning)
---   rw [← hTe]
---   rw [←NonSpanningCover_iff (T := T ) (X := Y ) (M := M ／ C)] at hT
---   have := (IsNonSpaningCover_contract_subset' hT hYne)
---   exact
---     Std.IsPreorder.le_trans (Y.coverNumber (M ↾ Y).Nonspanning) ((fun x ↦ x ∪ C) '' T).encard T.encard
---       ((IsNonSpaningCover_contract_subset hT hX hYne).coverNumber_le)
---       (encard_image_le (fun x ↦ x ∪ C) T )
-
-lemma NonSpanningNumber_set_closure (hY : Y ⊆ M.closure X) (hX : X ⊆ M.E) :
+lemma nonSpanningNumber_set_closure (hY : Y ⊆ M.closure X) (hX : X ⊆ M.E) :
     X.coverNumber (M ↾ X).Nonspanning  ≤ (X ∪ Y).coverNumber (M ↾ (X ∪ Y)).Nonspanning := by
   obtain hT | ⟨T, hT, hTe ⟩ := (X ∪ Y).exists_cover (M ↾ (X ∪ Y)).Nonspanning
   · rw [hT]
@@ -1199,1353 +1108,3 @@ lemma NonSpanningNumber_set_closure (hY : Y ⊆ M.closure X) (hX : X ⊆ M.E) :
   exact encard_image_le (fun x ↦ x ∩ X) T
 
 end NonSpanning
-
-
-
-
-
-
-
--- variable {α : Type*} {M N M' : Matroid α} {I F X Y F' F₀ F₁ F₂ P L H H₁ H₂ H' B C D K : Set α}
---   {e f : α} {l r : ℕ} {a k : ℕ∞} {T : Set (Set α)} {ι : Type*} {i j : ι}
---   {P P' : Matroid α → Set α → Prop}
-
--- section General
-
-
-
-
--- @[mk_iff]
--- structure IsCover (M : Matroid α) (P : Matroid α → Set α → Prop) (T : Set (Set α)) : Prop where
---   sUnion_eq : ⋃₀ T = M.E
---   pProp : ∀ F ∈ T, P M F
-
--- lemma IsCover.subset_ground (h : M.IsCover P T) (hX : X ∈ T) : X ⊆ M.E := by
---   grw [← h.sUnion_eq, ← subset_sUnion_of_mem hX]
-
--- -- monotone
--- -- PCover iff ∀ e, ∃ X ∈ T, e ∈ X
-
--- --Monotone under restriction
--- def IsMRProp (P : Matroid α → Set α → Prop) : Prop :=
---     ∀ M : Matroid α, ∀ F : Set α, ∀ Y : Set α, Y ⊆ F → P (M ↾ F) Y → P M Y
-
--- --Monotone under subset
--- def IsMSProp (P : Matroid α → Set α → Prop) : Prop :=
---     ∀ M : Matroid α, ∀ F : Set α, ∀ Y : Set α, Y ⊆ F → P M F → P M Y
-
--- -- --Minor union different prop. I think I want something different
--- -- def IsMUProp (P : Matroid α → Set α → Prop) (P' : Matroid α → Set α → Prop) : Prop :=
--- --     ∀ M : Matroid α, ∀ X : Set α, ∀ Y : Set α, P (M ／ X) Y → P' M (Y ∪ X)
-
--- --Minor monotono
--- -- def IsMMProp (P : Matroid α → Set α → Prop) (P' : Matroid α → Set α → Prop) : Prop :=
--- --     --∀ M : Matroid α, ∀ X : Set α, ∀ Y : Set α, P (M ／ X) Y → P' M (Y ∪ X)
--- --     ∀ N, N ≤m M → ∀ Y, Y ⊆ N.E → P N Y → P' M Y
-
--- -- M has a cover with respect to prop P
--- def hasCover_with (M : Matroid α) (P : Matroid α → Set α → Prop) : Prop :=
---     ∃ T, M.IsCover P T
-
--- lemma Cover_Nonempt_iff :
---     M.hasCover_with P ↔ {T | M.IsCover P T}.Nonempty := by
---   refine ⟨ fun a ↦ Nonempty.mono (fun ⦃a⦄ a_1 ↦ a_1) a , fun a ↦ ((fun a_1 ↦ a) ∘ fun a ↦ α) α ⟩
-
--- lemma IsCover.nonempty [M.Nonempty] (h : M.IsCover P T) : T.Nonempty := by
---   rw [nonempty_iff_empty_ne]
---   rintro rfl
---   simp [isCover_iff, eq_comm, M.ground_nonempty.ne_empty] at h
-
--- lemma IsCover.one_le [M.Nonempty] (h : M.IsCover P T) : 1 ≤ T.encard := by
---   simp only [one_le_encard_iff_nonempty]
---   exact nonempty h
-
--- noncomputable def coverNumber (M : Matroid α) (P : Matroid α → Set α → Prop) : ℕ∞ :=
---     sInf (encard '' {T | M.IsCover P T})
-
--- lemma coverNumber_eq_iInf (M : Matroid α) (P : Matroid α → Set α → Prop) :
---     M.coverNumber P = ⨅ T ∈ {T | M.IsCover P T}, T.encard := by
---   exact sInf_image
-
--- lemma IsCover.coverNumber_le {T} (h : M.IsCover P T) : M.coverNumber P ≤ T.encard := by
---   grw [coverNumber_eq_iInf]
---   exact biInf_le encard h
-
--- lemma exists_mincover_NE {M : Matroid α} {P : Matroid α → Set α → Prop}
---     (hn : {T | M.IsCover P T}.Nonempty) :
---     ∃ T, M.IsCover P T ∧ T.encard = M.coverNumber P := by
---   simpa using csInf_mem <| hn.image encard
-
--- lemma exists_min_cover {M : Matroid α} {P : Matroid α → Set α → Prop} (hP : M.hasCover_with P) :
---     ∃ T, M.IsCover P T ∧ T.encard = M.coverNumber P := by
---   simpa using csInf_mem <| (Cover_Nonempt_iff.1 hP ).image encard
-
--- lemma exists_cover (M : Matroid α) (P : Matroid α → Set α → Prop) :
---     M.coverNumber P = ⊤ ∨ ∃ T, M.IsCover P T ∧ T.encard = M.coverNumber P := by
---   obtain h0 | h := {T | M.IsCover P T}.eq_empty_or_nonempty
---   · simp [coverNumber_eq_iInf, h0]
---   right
---   simpa using csInf_mem <| h.image encard
-
--- lemma coverNumer_positive [M.Nonempty] (P : Matroid α → Set α → Prop) :
---     1 ≤ M.coverNumber P := by
---   by_contra hc
---   have h1 := ENat.lt_one_iff_eq_zero.mp (Std.not_le.mp hc)
---   obtain ht | ⟨T, hT, hTe ⟩ := exists_cover M P
---   · rw [h1] at ht
---     simp only [ENat.zero_ne_top] at ht
---   have := hT.nonempty
---   grind
-
--- lemma IsCover.cover_fun {M : Matroid α} {P' : Matroid α → Set α → Prop} (hP' : IsMRProp P')
---     (hcover : M.IsCover P T)
---     (f : Set α → Set (Set α) )
---     (hfun : ∀ X ∈ T, (M ↾ X).IsCover P' (f X)) :
---     M.IsCover P' ( ⋃ X ∈ T, f X ):= by
---   refine ⟨ ?_, ?_ ⟩
---   · rw[←hcover.sUnion_eq]
---     refine ext ?_
---     intro e
---     refine ⟨ ?_, ?_ ⟩
---     · intro he
---       simp only [ mem_sUnion, mem_iUnion] at he
---       obtain ⟨T', ⟨ X, ⟨hX, hT'X ⟩ ⟩, hee ⟩ := he
---       simp only [mem_sUnion]
---       refine ⟨ X ,⟨ hX , mem_of_subset_of_mem ((hfun X hX).subset_ground hT'X ) hee  ⟩ ⟩
---     intro he
---     simp only [mem_sUnion] at he
---     obtain ⟨X, hXT, heX⟩ := he
---     simp only [mem_sUnion, mem_iUnion]
---     have h1 : e ∈ (M ↾ ↑X).E := by exact mem_of_subset_of_mem (fun ⦃a⦄ a_1 ↦ a_1) heX
---     rw[←(hfun X hXT ).sUnion_eq] at h1
---     simp only [mem_sUnion] at h1
---     obtain ⟨X', hX', heX' ⟩ := h1
---     refine ⟨ X', ⟨⟨X, ⟨hXT, hX'⟩ ⟩, heX'⟩ ⟩
---   intro F hF
---   simp only [ mem_iUnion] at hF
---   obtain ⟨X, hXT, hF⟩ := hF
---   exact hP' M X F (LE.le.subset ((hfun X hXT).subset_ground hF ) ) ((hfun X hXT).pProp F hF)
-
-
--- lemma IsCover.cover_typset {P' : Matroid α → Set α → Prop} (hP' : IsMRProp P' )
---     (hcover : M.IsCover P T )
---     (f : T → Set (Set α) )
---     (hfun : ∀ X : T, (M ↾ X.1).IsCover P' (f X)) :
---     M.IsCover P' (⋃ X : T, f X ):= by
---   refine ⟨ ?_, ?_ ⟩
---   · rw[←hcover.sUnion_eq]
---     refine ext ?_
---     intro e
---     refine ⟨ ?_, ?_ ⟩
---     · intro he
---       simp only [iUnion_coe_set, mem_sUnion, mem_iUnion] at he
---       obtain ⟨T', ⟨ X, ⟨hX, hT'X ⟩ ⟩, hee ⟩ := he
---       simp only [mem_sUnion]
---       refine ⟨X, ⟨hX, (mem_of_subset_of_mem (((hfun ⟨X, hX⟩ ).subset_ground hT'X)) hee ) ⟩⟩
---     intro he
---     simp only [mem_sUnion] at he
---     obtain ⟨X, hXT, heX⟩ := he
---     simp only [iUnion_coe_set, mem_sUnion, mem_iUnion]
---     have h1 : e ∈ (M ↾ ↑X).E := by exact mem_of_subset_of_mem (fun ⦃a⦄ a_1 ↦ a_1) heX
---     rw[←(hfun ⟨X, hXT⟩ ).sUnion_eq] at h1
---     simp only [mem_sUnion] at h1
---     obtain ⟨X', hX', heX' ⟩ := h1
---     refine ⟨ X', ⟨⟨X, ⟨hXT, hX'⟩ ⟩, heX'⟩ ⟩
---   intro F hF
---   simp only [iUnion_coe_set, mem_iUnion] at hF
---   obtain ⟨X, hXT, hF⟩ := hF
---   exact hP' M X F (LE.le.subset ((hfun ⟨X, hXT⟩).subset_ground hF ) ) ((hfun ⟨X, hXT⟩).pProp F hF)
-
--- lemma coverNumber_cover_of_covers {P' : Matroid α → Set α → Prop} (hcover : M.IsCover P T)
---     (hP' : IsMRProp P') :
---     M.coverNumber P' ≤ ∑' X : T, (M ↾ X.1).coverNumber P' := by
---   obtain (h0 | h1) := exists_or_forall_not (fun X : T ↦ (M ↾ X).coverNumber P' = ⊤)
---   · simp [ENat.tsum_eq_top_of_eq_top h0]
---   have hf : ∀ X : T, ∃ XT, (M ↾ X.1).IsCover P' XT ∧
---     XT.encard = (M ↾ X.1).coverNumber P' := by
---     intro X
---     obtain (h | ⟨XT, hXres, hencard⟩) := (M ↾ X).exists_cover P'
---     · simp [h1 _ h]
---     exact ⟨XT, hXres, hencard⟩
---   choose f hfunco hfunca using hf
---   have hcover := IsCover.cover_typset hP' hcover f hfunco
---   grw [hcover.coverNumber_le, ENat.encard_iUnion_le_tsum_encard, tsum_congr hfunca]
-
--- lemma coverNumber_cover_of_covers_bound {P' : Matroid α → Set α → Prop} {k : ℕ∞}
---     (hcover : M.IsCover P T) (hP' : IsMRProp P')
---     (hflat : ∀ F, P M F → (M ↾ F).coverNumber P' ≤ k) :
---     M.coverNumber P' ≤ (T.encard) * k := by
---   grw [coverNumber_cover_of_covers hcover, ENat.tsum_le_tsum (g := fun _ ↦ k),
---     ENat.tsum_subtype_const, mul_comm]
---   intro F
---   simp [hflat _ <| hcover.pProp F F.2 ]
---   exact hP'
-
-
--- --P is minor preserved wrt f if
--- def MRProp (α) (P : Matroid α → Set α → Prop) (f : Set α → Matroid α → Set α → Prop ) : Prop :=
---     ∀ M : Matroid α, ∀ Y X : Set α,
---     ∃ (Q : Matroid α → Set α → Prop) , (P (M ／ Y) X → Q M X ∧ Q M X = f Y M X)
-
--- --Help
--- lemma RankIsMRProp (α) {k : ℕ∞} : MRProp (α)
---     (fun M X ↦ M.eRk X ≤ k) (fun Y M X ↦ M.eRk (X ∪ Y) ≤ M.eRk Y + k ) := by
---   intro M Y X
---   use (fun N Z ↦ M.eRk (X ∪ Y) ≤ M.eRk Y + k )
---   simp only [and_true]
-
---   sorry
-
--- -- --Minor preserved under f
--- -- --(f : Set α → Matroid α → (Set α → Prop))
--- -- def IsMUProp (P : Matroid α → Set α → Prop) (X : Set α ) (P' : Matroid α → Set α → Prop): Prop :=
--- --     --∀ X : Set α,
--- --     --∃ P' : Matroid α → Set α → Prop,
--- --     ∀ M : Matroid α,
--- --     ∀ Y : Set α, P (M ／ X) Y → P' M Y
-
--- --P ' = k + M.eRk X for rank
--- lemma IsCover.contract (h : (M ／ X).IsCover P T)
---     (hX : X ⊆ M.E) (hXN : (M ／ X).Nonempty)
---     (hPP' : ∀ Y : Set α, P (M ／ X) Y → P' M ( Y ∪ X) ) :
---     M.IsCover P' ((· ∪ X) '' T) := by
---   suffices hi : ∀ F ∈ T, P (M ／ X) F by
---     simp only [isCover_iff, sUnion_image, mem_image, forall_exists_index, and_imp,
---       forall_apply_eq_imp_iff₂, ← biUnion_distrib_union _ h.nonempty, ← sUnion_eq_biUnion,
---       h.sUnion_eq, contract_ground, diff_union_self, union_eq_left, hX, true_and ]
---     exact fun F hFT ↦ (((fun a ↦ (hPP' F (hi F hFT))) ∘ T) X )
---   exact fun F hFT ↦ h.pProp F hFT
-
-
--- --Close under closure
--- def IsCCProp (α) (P : Matroid α → Set α → Prop) : Prop :=
---     ∀ M : Matroid α, ∀ F : Set α, P M F → P M (M.closure F)
-
--- lemma IsCover.isCover_closure (h : M.IsCover P T) (hP : IsCCProp α P) :
---     M.IsCover P (M.closure '' T) := by
---   simp only [isCover_iff, sUnion_image, subset_antisymm_iff (b := M.E), iUnion_subset_iff,
---     M.closure_subset_ground, implies_true, true_and, mem_image, forall_exists_index, and_imp,
---     forall_apply_eq_imp_iff₂]
---   grw [h.sUnion_eq.symm.subset, sUnion_eq_biUnion]
---   refine  ⟨biUnion_mono rfl.subset fun X hX ↦ M.subset_closure X (h.subset_ground hX),
---   fun F hF ↦ (hP M F (h.pProp F hF)) ⟩
-
--- --Singleton section
--- -- noncomputable def SetsingletonEmbedding ( A : Set α ) : Function.Embedding
--- --     {X : Set α // ∃ e ∈ A, {e} = X} {e // e ∈ A} :=
--- -- { toFun := fun x => ⟨Classical.choose x.2, (Classical.choose_spec x.2).1 ⟩
--- --   inj' := by
--- --     intro x y hxy
--- --     simp only [Subtype.mk.injEq] at hxy
--- --     have heq : x.1 = y.1 := by
--- --       rw [←(Classical.choose_spec x.2).2, ←(Classical.choose_spec y.2).2]
--- --       exact singleton_eq_singleton_iff.mpr hxy
--- --     exact Subtype.ext heq
--- --     }
-
--- lemma IsCover_singleton_Prop (hP : ∀ e ∈ M.E, P M (singleton e)) :
---     M.IsCover P (singleton '' M.E) := by
---   refine ⟨ ?_, ?_ ⟩
---   · refine Eq.symm (ext ?_)
---     intro x
---     refine ⟨ ?_, ?_ ⟩
---     · intro hx
---       refine mem_sUnion.mpr ⟨{x} , ⟨ ?_ , mem_singleton x ⟩ ⟩
---       use x
---     intro hc
---     simp only [sUnion_image, biUnion_of_singleton] at hc
---     exact mem_of_subset_of_mem (fun ⦃a⦄ a_1 ↦ a_1) hc
---   intro F hF
---   obtain ⟨e, heE, heF ⟩ := hF
---   rw[←heF]
---   exact hP e heE
-
-
--- lemma IsCover_singleton_le (hP : ∀ e ∈ M.E, P M (singleton e)) :
---     M.coverNumber P ≤ M.E.encard := by
---   grw [(IsCover_singleton_Prop hP).coverNumber_le ]
---   set Sing : Set (Set α ) := { singleton e | e ∈ M.E} with hs
---   exact encard_image_le singleton M.E
-
-
--- lemma IsCover.mono_prop (h : M.IsCover P T) (hPP' : ∀ X ∈ T, P M X → P' M X) : M.IsCover P' T :=
---   (M.isCover_iff P' T).2 ⟨h.sUnion_eq, fun F hF ↦ hPP' F hF (h.pProp F hF)⟩
-
--- lemma IsCover_emptyset_iff (P : Matroid α → Set α → Prop) : M.IsCover P ∅ ↔ ¬M.Nonempty := by
---   refine ⟨?_, ?_ ⟩
---   · intro h
---     rw [ ←Matroid.ground_nonempty_iff, not_nonempty_iff_eq_empty, ←sUnion_empty, h.sUnion_eq.symm ]
---   intro h
---   rw [ ←Matroid.ground_nonempty_iff, not_nonempty_iff_eq_empty, ←sUnion_empty] at h
---   refine ⟨h.symm, by grind ⟩
-
--- lemma coverNumber_zero_iff (P : Matroid α → Set α → Prop) : M.coverNumber P = 0 ↔ M.IsCover P ∅ := by
---   refine ⟨?_, ?_ ⟩
---   · intro h
---     obtain ht | ⟨T, hT, hTe ⟩ := exists_cover M P
---     · by_contra
---       rw[ht] at h
---       simp only [ENat.top_ne_zero] at h
---     rw [h] at hTe
---     rwa [← encard_eq_zero.mp hTe  ]
---   intro h
---   have := h.coverNumber_le
---   simp only [encard_empty, nonpos_iff_eq_zero] at this
---   grind
-
--- -- lemma coverNumber_le_coverNumber (P Q : Matroid α → Set α → Prop) (M : Matroid α)
--- --     (hPQ : ∀ X ⊆ M.E, P M X → Q M X) : M.coverNumber Q ≤ M.coverNumber P := by
--- --   sorry
-
--- -- lemma coverNumber_congr (P Q : Matroid α → Set α → Prop)
--- --     (hPQ : ∀ (M : Matroid α) (X : Set α), X ⊆ M.E → (P M X ↔ Q M X)) (M : Matroid α) :
--- --     M.coverNumber P = M.coverNumber Q := by
--- --   sorry
-
--- -- lemma coverNumber_mono_prop (P : Matroid α → Set α → Prop) {M N : Matroid α} (hMN : M.E = N.E)
--- --     (hMP : ∀ X ⊆ M.E, P N X → P M X) : M.coverNumber P ≤ N.coverNumber P := by
-
--- --   simp only [coverNumber, le_sInf_iff, mem_image, mem_setOf_eq, forall_exists_index, and_imp,
--- --     forall_apply_eq_imp_iff₂]
--- --   refine fun C hC ↦ sInf_le ?_
--- --   simp only [mem_image, mem_setOf_eq]
--- --   refine ⟨C, ?_, rfl⟩
--- --   have := hC.mono_prop (P' := P)
-
-
--- end General
-
--- section Rank
-
--- -- lemma RankPropIsMUProp {k : ℕ∞} : IsMUProp (RankProp α k) (fun M X Y ↦ (M.eRk Y ≤ k + M.eRk X)) := by
--- --     --use fun M X Y ↦ (M.eRk Y ≤ k + M.eRk X)
--- --     intro M X Y hXY
--- --     unfold RankProp at hXY
--- --     sorry
-
--- def IsRankCover (M : Matroid α) (k : ℕ∞) (T : Set (Set α )) : Prop :=
---     M.IsCover (fun M X ↦ M.eRk X ≤ k) T
-
--- lemma IsRankCover_iff_IsCover (M : Matroid α) (k : ℕ∞) (T : Set (Set α )) :
---     M.IsRankCover k T ↔ M.IsCover (fun M X ↦ M.eRk X ≤ k) T := Iff.rfl
-
--- lemma IsRankCover_iff (M : Matroid α) (k : ℕ∞) (T : Set (Set α )) :
---     M.IsRankCover k T ↔ ⋃₀ T = M.E ∧ (∀ F ∈ T, M.eRk F ≤ k) := by
---   sorry
---   --Mathieu
-
--- lemma IsRankCover_isCover_closure (hcov : M.IsRankCover k T) :
---     M.IsRankCover k (M.closure '' T) := by
---   apply hcov.isCover_closure (fun M F hF ↦ ?_)
---   rwa [(eRk_closure_eq M F) ]
-
--- lemma IsRankCover.mono_k {k' : ℕ∞} (hcov : M.IsRankCover k T) (hkk' : k ≤ k') :
---     M.IsRankCover k' T := by
---   refine ⟨ hcov.sUnion_eq, fun F hF ↦
---     Std.IsPreorder.le_trans (M.eRk F) k k' (hcov.pProp F hF ) hkk' ⟩
-
--- lemma IsRankCover_RankPos : M.hasCover_with (fun M X ↦ M.eRk X ≤ 0) ↔ ¬ M.RankPos := by
---   refine ⟨ ?_, ?_ ⟩
---   · intro h
---     refine M.not_rankPos_iff.2 (Matroid.eq_loopyOn_iff_loops.mpr
---       ⟨Eq.symm (Subset.antisymm ?_ (loops_subset_ground M )) , by simp only ⟩   )
---     intro e he
---     obtain ⟨ T, hT ⟩ := h
---     rw[←hT.sUnion_eq ] at he
---     obtain ⟨ X, hXt, heX ⟩ := he
---     exact isLoop_iff.mp (((Matroid.eRk_eq_zero_iff (IsCover.subset_ground hT hXt  )).1
---       (nonpos_iff_eq_zero.mp (hT.pProp X hXt ))) heX)
---   intro h
---   refine ⟨ (singleton '' M.E), IsCover_singleton_Prop ?_ ⟩
---   intro e he
---   simp only [nonpos_iff_eq_zero]
---   refine IsLoop.eRk_eq ?_
---   rw [M.not_rankPos_iff.1 h]
---   exact loopyOn_isLoop_iff.mpr he
-
--- lemma IsRankCover_two [M.Nonempty] (hcov : M.IsRankCover k T) (hk : k < M.eRank ) :
---     2 ≤ T.encard := by
---   by_contra hc
---   simp only [not_le] at hc
---   have hle : T.encard ≤ 1 := Order.le_of_lt_succ hc
---   have h1 := ((IsRankCover_iff_IsCover M k T).1 hcov).one_le
---   have h1 : T.encard = 1 := by grind
---   obtain ⟨X, hX ⟩ := Set.encard_eq_one.1 h1
---   have h2 := ((IsRankCover_iff_IsCover M k T).1 hcov).sUnion_eq
---   rw [hX] at h2
---   simp only [sUnion_singleton] at h2
---   have hXT : X ∈ T := by
---     rw[ hX ]
---     exact mem_singleton X
---   have hf := ((IsRankCover_iff_IsCover M k T).1 hcov).pProp X hXT
---   rw[ h2, ←eRank_def M  ] at hf
---   grind
-
-
--- lemma setOf_point_IsRankCover (M : Matroid α) [M.RankPos] : M.IsRankCover 1 {P | M.IsPoint P} := by
---   refine ⟨subset_antisymm (sUnion_subset fun _ ↦ IsPoint.subset_ground) fun e he ↦ ?_,
---     by simp +contextual [mem_setOf_eq, IsPoint] ⟩
---   simp only [mem_sUnion, mem_setOf_eq]
---   obtain hl | hnl := M.isLoop_or_isNonloop e
---   · obtain ⟨f, hf⟩ := M.exists_isNonloop
---     exact ⟨_, hf.closure_isPoint, hl.mem_closure _⟩
---   exact ⟨_, hnl.closure_isPoint, mem_closure_of_mem _ (by simp) (by simpa)⟩
-
--- lemma setOf_point_IsCover [hM : M.Loopless] : M.IsRankCover 1 {P | M.IsPoint P} := by
---   obtain ⟨E, rfl⟩ | h := M.eq_loopyOn_or_rankPos'
---   · obtain rfl : E = ∅ := by simpa using hM
---     constructor <;> simp [IsPoint]
---   exact M.setOf_point_IsRankCover
-
--- lemma IsRankCover_ground (M : Matroid α) : M.IsRankCover M.eRank ({M.E}) := by
---   refine ⟨ by simp, fun F a ↦ eRk_le_eRank M F ⟩
-
--- lemma IsRankCover.nonempty [M.Nonempty] (h : M.IsRankCover k T) : T.Nonempty := by
---   rw [nonempty_iff_empty_ne]
---   rintro rfl
---   simp [IsRankCover_iff, eq_comm, M.ground_nonempty.ne_empty] at h
-
--- lemma RankPropCover_exists (hk : 1 ≤ k) : M.hasCover_with (fun M X ↦ M.eRk X ≤ k) := by
---   by_cases hRP : M.RankPos
---   · refine ⟨{P | M.IsPoint P}, (setOf_point_IsRankCover M ).mono_k hk ⟩
---   obtain ⟨ T, hT ⟩ := IsRankCover_RankPos.2 hRP
---   refine ⟨ T, ((IsRankCover_iff_IsCover M 0 T).2 hT).mono_k (ENat.zero_le ) ⟩
-
--- lemma IsCover.delete (hT : M.IsCover (fun M X ↦ M.eRk X ≤ k) T) (D : Set α) :
---     (M ＼ D).IsCover (fun M X ↦ M.eRk X ≤ k) ((fun s ↦ s \ D) '' T) := by
---   refine ⟨ ?_, ?_ ⟩
---   · refine subset_antisymm (sUnion_subset fun K ↦ ?_) fun e he ↦ ?_
---     · intro hK
---       obtain ⟨ X, hX, h ⟩ := hK
---       rw[ ← h]
---       exact diff_subset_diff_left (hT.subset_ground hX )
---     simp only [delete_ground, mem_diff] at he
---     rw [←hT.sUnion_eq] at he
---     obtain ⟨X, hX, hXe ⟩ := he.1
---     have : e ∈ X \ D := mem_diff_of_mem hXe (he.2 )
---     grind
---   intro F hF
---   obtain ⟨ F' ,hF' ,hF2 ⟩ := hF
---   rw [←hF2]
---   simp only [delete_eRk_eq', sdiff_idem]
---   grw [eRk_subset_le M (diff_subset)]
---   exact hT.pProp F' hF'
-
--- --Help
--- lemma coverNumber_eRank [M.Nonempty] : M.coverNumber (fun M' X ↦ M'.eRk X ≤ M.eRank) = 1 := by
---   have h2 : 1 ≤ M.coverNumber (fun M' X ↦ M'.eRk X ≤ M.eRank ) :=
---     M.coverNumer_positive (fun M' X ↦ M'.eRk X ≤ M.eRank )
---   refine h2.antisymm' ?_
---   simpa using (IsRankCover_ground M).coverNumber_le
-
--- -- lemma coverNumber_delete_loop (hne : (M ＼ D).Nonempty) (hk : 1 ≤ k) (hD : D ⊆ M.loops ) :
--- --     M.coverNumber (fun M X ↦ M.eRk X ≤ k) = (M ＼ D).coverNumber (fun M X ↦ M.eRk X ≤ k) := by
--- --   obtain ⟨T, hT, hTen ⟩ := exists_min_cover (RankPropCover_exists (M := M) hk )
--- --   have h1 := (hT.delete D ).coverNumber_le
--- --   grw[encard_image_le (fun s ↦ s \ D) T, hTen ] at h1
--- --   -- have hkD : (M ＼ D).RankPos := by
--- --   --   have hh : (M ＼ M.loops).RankPos := Delete_loops_RankPos
--- --   --   rw [Matroid.rankPos_iff ] at hh
--- --   --   simp only [delete_isBase_iff] at hh
--- --   --   refine { empty_not_isBase := ?_ }
--- --   --   by_contra hc
--- --   --   exact Ne.elim (fun a ↦ hh ((((Matroid.IsBasis.isBasis_subset (isBasis_ground_iff.mpr hc )
--- --   --   (empty_subset (M.E \ D) ) (IsLoopEquiv.subset_ground rfl fun ⦃a⦄ a_1 ↦ a_1) ) ).isBasis_subset
--- --   --     (empty_subset (M.E \ M.loops) ) (diff_subset_diff_right hD ) ).of_delete)) hTen
--- --   --have : (M ＼ D).Nonempty := rankPos_nonempty
--- --   obtain ⟨T', hT', hT'en ⟩ := exists_min_cover (RankPropCover_exists (M := (M ＼ D)) hk )
--- --   have hcov : M.IsCover (fun M X ↦ M.eRk X ≤ k) (M.closure '' T' ) := by
--- --     refine ⟨ ?_, ?_ ⟩
--- --     · refine subset_antisymm (sUnion_subset fun K ↦ ?_) fun e he ↦ ?_
--- --       · simp only [mem_image, forall_exists_index, and_imp]
--- --         grind
--- --       by_cases heD : e ∈ D
--- --       · obtain ⟨ X, hX ⟩ := hT'.nonempty
--- --         have := (IsLoop.mem_closure (hD heD) X )
--- --         grind
--- --       have h2 : e ∈ M.E \ D := mem_diff_of_mem he heD
--- --       rw[←delete_ground,  ←hT'.sUnion_eq  ] at h2
--- --       obtain ⟨ X, hX, heX ⟩ := h2
--- --       have := (mem_closure_of_mem' M heX he )
--- --       grind
--- --     intro F hF
--- --     obtain ⟨F' ,hF', hF2 ⟩ := hF
--- --     rw[←hF2, eRk_closure_eq M F']
--- --     have ha := hT'.pProp F' hF'
--- --     simp only [delete_eRk_eq'] at ha
--- --     have ha1 : F' \ D = F' := by
--- --       have := hT'.subset_ground hF'
--- --       grind
--- --     rwa [ha1] at ha
--- --   have h2 := hcov.coverNumber_le
--- --   grw [encard_image_le M.closure T', hT'en] at h2
--- --   grind
-
--- -- lemma coverNumber_contract_loop (hne : (M ＼ D).Nonempty) (hk : 1 ≤ k) (hD : D ⊆ M.loops ) :
--- --     M.coverNumber (fun M X ↦ M.eRk X ≤ k) = (M ／ D).coverNumber (fun M X ↦ M.eRk X ≤ k) := by
--- --   rw[contract_eq_delete_of_subset_loops hD]
--- --   exact coverNumber_delete_loop hne hk hD
-
--- -- lemma IsRankCover.contract (h : (M ／ X).IsRankCover k T) (hX : X ⊆ M.E)
--- --     (hXN : (M ／ X).Nonempty) :
--- --     M.IsRankCover (k + M.eRk X) ((· ∪ X) '' T) := by
--- --   suffices ∀ F ∈ T, M.eRk (F ∪ X) ≤ k + M.eRk X by
--- --     simpa [IsRankCover_iff, ← biUnion_distrib_union _ h.nonempty, ← sUnion_eq_biUnion, h.sUnion_eq, hX]
--- --   exact fun F hFT ↦ by grw [← h.pProp F hFT, ← eRelRk_eq_eRk_contract, eRelRk_add_eRk_eq]
-
--- -- lemma coverNumber_contract_one {a : ℕ∞} (he : e ∈ M.E) (hel : M.IsNonloop e)
--- --     (heN : (M／ {e}).Nonempty) :
--- --     M.coverNumber (fun M X ↦ M.eRk X ≤ (a + 1)) ≤ (M ／ {e}).coverNumber (fun M X ↦ M.eRk X ≤ a)
--- --     := by
--- --   refine ENat.forall_natCast_le_iff_le.mp ?_
--- --   intro b hb
--- --   unfold coverNumber at hb
--- --   simp only [le_sInf_iff, mem_image, mem_setOf_eq, forall_exists_index, and_imp,
--- --     forall_apply_eq_imp_iff₂] at hb
--- --   unfold coverNumber
--- --   simp only [le_sInf_iff, mem_image, mem_setOf_eq, forall_exists_index, and_imp,
--- --     forall_apply_eq_imp_iff₂]
--- --   intro T hT
--- --   rw[←IsRankCover_iff_IsCover] at hT
--- --   have h1 := hT.contract (singleton_subset_iff.mpr he ) heN
--- --   rw[IsNonloop.eRk_eq hel ] at h1
--- --   have h2 := hb ((· ∪ {e}) '' T) h1
--- --   grw[encard_image_le (fun x ↦ x ∪ {e}) T ] at h2
--- --   exact h2
-
--- -- lemma exists_cover (M : Matroid α) {k : ℕ∞} (hk : 1 ≤ k) :
--- --     ∃ T, M.IsCover k T ∧ T.encard = M.coverNumber k := by
--- --   simpa using csInf_mem <| (M.setOf_cover_nonempty hk).image encard
-
-
-
--- -- lemma coverNumber_contract {a : ℕ∞} (hX : X ⊆ M.E) :
--- --     M.coverNumber (a + M.eRk X) ≤ (M ／ X).coverNumber a := by
--- --   --Mathieu, do you want to do this one?
--- --   sorry
-
--- -- def closZ (a : ℕ) (hx : X.Finite ) (hX : X ⊆ M.E)
--- --     (Y : (M ↾ F).closure '' { Y | Y ⊆ X ∧ M.eRk Y = a} )
--- --     : ∃ Z :  { Y | Y ⊆ X ∧ M.eRk Y = a}, Y.1 = Z.1 := by
--- --   have := (mem_image ((M ↾ F).closure) ({ Y | Y ⊆ X ∧ M.eRk Y = a}) Y.1  ).1 Y.2
--- --   obtain ⟨Y, hY ⟩ := (mem_image ((M ↾ F).closure) ({ Y | Y ⊆ X ∧ M.eRk Y = a}) Y.1  ).1 Y.2
--- --   sorry
-
--- -- def IsFlat.restriction_clo (hF : M.IsFlat F) (hY : Y ⊆ F) : M.closure Y = (M ↾ F).closure Y :=
--- --     by
--- --   sorry
-
-
-
--- --Dont need
--- -- def closZ (a : ℕ)
--- --     (Z : (M ↾ F).closure '' { Y | Y ⊆ X ∧ M.eRk Y = a} )
--- --     : ∃ Y :  { Y | Y ⊆ X ∧ M.eRk Y = a}, (M ↾ F).closure Y.1 = Z.1 := by
--- --   --have := (mem_image ((M ↾ F).closure) ({ Y | Y ⊆ X ∧ M.eRk Y = a}) Y.1  ).1 Y.2
--- --   obtain ⟨Y, hY, h ⟩ := (mem_image ((M ↾ F).closure) ({ Y | Y ⊆ X ∧ M.eRk Y = a}) Z.1  ).1 Z.2
--- --   use ⟨Y, hY⟩
-
--- -- def getI (a : ℕ) (hX : X ⊆ M.E)
--- --     (Y : { Y | Y ⊆ X ∧ M.eRk Y = a} )
--- --     : ∃ I : {Y | Y ⊆ X ∧ Y.encard = a}, I.1 ⊆ X ∧ (M.IsBasis I Y.1) ∧ I.1.encard = a := by
--- --   --have : Y ⊆ M.E := by sorry
--- --   obtain ⟨I, hIB, hc ⟩ := (M.eq_eRk_iff.1 Y.2.2)
--- --   have h' :  I ∈ {Y | Y ⊆ X ∧ Y.encard = ↑a} := by
--- --     refine ⟨LE.le.subset fun ⦃a⦄ a_2 ↦ (Y.2.1 ) (IsBasis.subset hIB  a_2) , hc ⟩
--- --   use ⟨ I, h' ⟩
--- --   refine ⟨h'.1, hIB , hc ⟩
-
--- -- def ranksubsets_Map (a : ℕ) (b : ℕ) (hx : X.Finite ) (hX : X ⊆ M.E) (hF : M.IsFlat F) (hXF : X ⊆ F)
--- --     : Function.Embedding
--- --     ((M ↾ F).closure '' { Y | Y ⊆ X ∧ M.eRk Y = a}) {Y | Y ⊆ X ∧ Y.encard = a} :=
--- -- --have := LE.le.subset fun ⦃a⦄ a_1 ↦ hX (hY.1 a_1)
--- -- { toFun := fun Z =>
--- --     ⟨ (Classical.choose (getI a hX (Classical.choose (closZ a Z ))) ).1 ,
--- --     (Classical.choose (getI a hX (Classical.choose (closZ a Z ))) ).2 ⟩
--- --   inj' := by
--- --     intro x y hxy
--- --     simp only [Subtype.mk.injEq] at hxy
--- --     have heq : x.1 = y.1 := by
--- --       rw[ ←(Classical.choose_spec (closZ a x )), ←(Classical.choose_spec (closZ a y )) ]
--- --       --simp only [mem_setOf_eq, coe_setOf ]
--- --       rw[←hF.restriction_clo ?_, ←hF.restriction_clo ?_,
--- --       ←((Classical.choose_spec (getI a hX (Classical.choose (closZ a x ))) ).2.1).closure_eq_closure,
--- --       ←((Classical.choose_spec (getI a hX (Classical.choose (closZ a y ))) ).2.1).closure_eq_closure,
--- --       hxy ]
--- --       --simp only [restrict_closure_eq']
--- --       --have := (Classical.choose_spec (getI a hX (Classical.choose (closZ a x ))) ).1
--- --       have := (Classical.choose (closZ a x )).2.1
--- --       --exact LE.le.subset fun ⦃b⦄ b_2 ↦ hXF (this b_2)
--- --       --grw[hXF] at this
--- --       --intro Y hY
-
--- --       --simp only [mem_setOf_eq, coe_setOf] at this
-
--- --       sorry
--- --       · sorry
--- --     exact SetCoe.ext heq
--- --     --rw[ ] at hxy
-
--- --     }
-
--- lemma set_to_binom_number {a b : ℕ} (X : Set α) (hX : X.encard = b) :
---     {Y | Y ⊆ X ∧ Y.encard = a}.encard = b.choose a := by
---   have hXfin : X.Finite := by simp [← encard_lt_top_iff, hX]
---   set X' := hXfin.toFinset with hX'
---   have := (ENat.coe_inj).2 <| X'.card_powersetCard a
---   convert (ENat.coe_inj).2 <| X'.card_powersetCard a
---   · rw [← encard_coe_eq_coe_finsetCard, ← Finset.coe_injective.encard_image (β := Set α)]
---     convert rfl
---     ext S
---     simp only [mem_image, SetLike.mem_coe, Finset.mem_powersetCard, mem_setOf_eq,
---       hX', Finite.subset_toFinset]
---     constructor
---     · rintro ⟨T, ⟨hTX, rfl⟩, rfl⟩
---       simpa
---     intro ⟨hSX, hSa⟩
---     refine ⟨Finite.toFinset (s := S) ?_, ?_⟩
---     · simp [← encard_lt_top_iff, hSa]
---     simp_rw [← ENat.coe_inj, ← hSa, ← Finite.encard_eq_coe_toFinset_card]
---     simpa
---   rw [← ENat.coe_inj, ← hX, eq_comm, hXfin.encard_eq_coe_toFinset_card]
-
--- -- lemma base_isCover {a : ℕ} (hr : M.eRank ≤ a + 1) (ha : 1 ≤ a) (hXfin : X.Finite)
--- --     --(h : Maximal (fun Y ↦ Y ⊆ M.E ∧ (M ↾ Y).IsFiniteRankUniform (a + 1) Y.encard) X) :
--- --     (h : MaximalFor (fun x ↦ x ∈ {X | X ⊆ M.E ∧ (M ↾ X).IsFiniteRankUniform (a + 1) X.encard}) encard X) :
--- --     M.IsRankCover a (M.closure '' {K | K ⊆ X ∧ K.encard = a}) := by
--- --   refine ⟨?_, ?_⟩
--- --   · refine subset_antisymm (sUnion_subset fun K ↦ ?_) fun e he ↦ ?_
--- --     · simp only [mem_image, mem_setOf_eq, forall_exists_index, and_imp]
--- --       grind
--- --     obtain ⟨E, hEX, hEunif⟩ := h.prop.2.exists_eq_unifOn
--- --     obtain rfl : X = E := congr_arg Matroid.E hEunif
--- --     by_contra! hcon
--- --     simp only [sUnion_image, mem_setOf_eq, mem_iUnion, exists_prop, not_exists, not_and,
--- --       and_imp] at hcon
--- --     have hcon' (Z) (hZ : Z ⊆ X) (hZa : Z.encard ≤ a) : e ∉ M.closure Z := by
--- --       have haX : a ≤ X.encard := by
--- --         grw [← M.restrict_ground_eq (R := X), ← eRank_le_encard_ground, h.prop.2.eRank_eq]
--- --         simp
--- --       obtain ⟨W, hZW, hWZ, hW⟩ := exists_superset_subset_encard_eq hZ hZa haX
--- --       exact notMem_subset (M.closure_subset_closure hZW) (hcon W hWZ hW)
--- --     have heX : e ∉ X := by
--- --       by_contra hc
--- --       exact hcon' (singleton e) (singleton_subset_iff.mpr hc )
--- --         (by simp only [encard_singleton, ENat.one_le_coe, ha ]) (mem_closure_self M e he )
--- --     --have hwin := h.not_prop_of_ssuperset (t := insert e X) (by grind)
--- --     have hwin := h.not_prop_of_gt (j := insert e X)
--- --       (Finite.encard_lt_encard hXfin (ssubset_insert heX ))
--- --     simp only [mem_setOf_eq, not_and, insert_subset_iff.mpr ⟨he, h.prop.1 ⟩,forall_const ] at hwin
--- --     --rw [insert_subset_iff , and_iff_right he, and_iff_right h.prop.1] at hwin
--- --     apply hwin
--- --     suffices aux : (M ↾ insert e X) = unifOn (insert e X) (a + 1) by
--- --       rw [aux]
--- --       apply unifOn_isFiniteRank_uniform
--- --       grw [h.prop.2.le, ← subset_insert]
--- --     refine ext_indep rfl fun I (hI : I ⊆ insert e X) ↦ ?_
--- --     simp only [restrict_indep_iff, hI, and_true, unifOn_indep_iff, Nat.cast_add, Nat.cast_one]
--- --     refine ⟨fun hIi ↦ by grw [hIi.encard_le_eRank, hr], fun hcard ↦ ?_⟩
--- --     have hI₀ : M.Indep (I \ {e}) := by
--- --       have hrestr := (M.restrict_indep_iff (R := X) (I := I \ {e})).1
--- --       nth_grw 1 [hEunif, unifOn_indep_iff, diff_subset] at hrestr
--- --       grind
--- --     by_cases! heI : e ∉ I
--- --     · rwa [diff_singleton_eq_self heI] at hI₀
--- --     rw [← insert_diff_self_of_mem heI, hI₀.insert_indep_iff_of_notMem (by grind), mem_diff,
--- --       and_iff_right he]
--- --     refine hcon'  _ (by grind) ?_
--- --     grw [← ENat.add_one_le_add_one_iff, ← hcard, encard_diff_singleton_add_one heI]
--- --   simp only [mem_image, mem_setOf_eq, forall_exists_index, and_imp]
--- --   rintro F I hI hcard rfl
--- --   grw [eRk_closure_eq, eRk_le_encard, hcard]
-
--- lemma base_isCover {a : ℕ} (hr : M.eRank ≤ a + 1) (ha : 1 ≤ a) (hXfin : X.Finite)
---     --(h : Maximal (fun Y ↦ Y ⊆ M.E ∧ (M ↾ Y).IsFiniteRankUniform (a + 1) Y.encard) X) :
---     (h : MaximalFor (fun x ↦ x ∈ {X | X ⊆ M.E ∧ (M ↾ X).IsFiniteRankUniform (a + 1) }) encard X) :
---     M.IsRankCover a (M.closure '' {K | K ⊆ X ∧ K.encard = a}) := by
---   refine ⟨?_, ?_⟩
---   · refine subset_antisymm (sUnion_subset fun K ↦ ?_) fun e he ↦ ?_
---     · simp only [mem_image, mem_setOf_eq, forall_exists_index, and_imp]
---       grind
---     obtain ⟨E, hEX, hEunif⟩ := h.prop.2.exists_eq_unifOn
---     --obtain rfl : X = E := congr_arg Matroid.E hEunif
---     by_contra! hcon
---     simp only [sUnion_image, mem_setOf_eq, mem_iUnion, exists_prop, not_exists, not_and,
---       and_imp] at hcon
---     have hcon' (Z) (hZ : Z ⊆ X) (hZa : Z.encard ≤ a) : e ∉ M.closure Z := by
---       have haX : a ≤ X.encard := by
---         grw [← M.restrict_ground_eq (R := X), ← eRank_le_encard_ground, h.prop.2.eRank_eq]
---         simp
---       obtain ⟨W, hZW, hWZ, hW⟩ := exists_superset_subset_encard_eq hZ hZa haX
---       exact notMem_subset (M.closure_subset_closure hZW) (hcon W hWZ hW)
---     have heX : e ∉ X := by
---       by_contra hc
---       exact hcon' (singleton e) (singleton_subset_iff.mpr hc )
---         (by simp only [encard_singleton, ENat.one_le_coe, ha ]) (mem_closure_self M e he )
---     --have hwin := h.not_prop_of_ssuperset (t := insert e X) (by grind)
---     have hwin := h.not_prop_of_gt (j := insert e X)
---       (Finite.encard_lt_encard hXfin (ssubset_insert heX ))
---     simp only [mem_setOf_eq, not_and, insert_subset_iff.mpr ⟨he, h.prop.1 ⟩,forall_const ] at hwin
---     --rw [insert_subset_iff , and_iff_right he, and_iff_right h.prop.1] at hwin
---     apply hwin
---     suffices aux : (M ↾ insert e X) = unifOn (insert e X) (a + 1) by
---       rw [aux]
---       apply unifOn_isFiniteRankUniform
---       grw [h.prop.2.le , ← subset_insert]
---       exact encard_le_encard fun ⦃a⦄ a_1 ↦ a_1
---     refine ext_indep rfl fun I (hI : I ⊆ insert e X) ↦ ?_
---     simp only [restrict_indep_iff, hI, and_true, unifOn_indep_iff, Nat.cast_add, Nat.cast_one]
---     refine ⟨fun hIi ↦ by grw [hIi.encard_le_eRank, hr], fun hcard ↦ ?_⟩
---     have hI₀ : M.Indep (I \ {e}) := by
---       have hrestr := (M.restrict_indep_iff (R := X) (I := I \ {e})).1
---       have : I \ {e} ⊆ E  := by
---         rw [ ←unifOn_ground_eq E (k := a + 1), ← hEX, restrict_ground_eq, diff_subset_iff, singleton_union]
---         exact LE.le.subset hI
---       nth_grw 1 [hEX, unifOn_indep_iff, diff_subset] at hrestr
---       grind
---     by_cases! heI : e ∉ I
---     · rwa [diff_singleton_eq_self heI] at hI₀
---     rw [← insert_diff_self_of_mem heI, hI₀.insert_indep_iff_of_notMem (by grind), mem_diff,
---       and_iff_right he]
---     refine hcon'  _ (by grind) ?_
---     grw [← ENat.add_one_le_add_one_iff, ← hcard, encard_diff_singleton_add_one heI]
---   simp only [mem_image, mem_setOf_eq, forall_exists_index, and_imp]
---   rintro F I hI hcard rfl
---   grw [eRk_closure_eq, eRk_le_encard, hcard]
-
--- lemma baseCase {a b : ℕ} (ha : 1 ≤ a) (hM : NoUniformMinor M (a + 1) (b + 1))
---     (hr : M.eRank = a + 1) :
---     M.coverNumber (fun M X ↦ M.eRk X ≤ a) ≤ Nat.choose b a := by
---   have : M.RankFinite := M.eRank_ne_top_iff.mp (ENat.ne_top_iff_exists.2
---       (Exists.intro ((fun x1 x2 ↦ x1 + x2) a 1) (hr.symm)))
---   by_contra! hcon
---   obtain ⟨B, hB⟩ := M.exists_isBase
---   set Unif : Set (Set α) := {X | X ⊆ M.E ∧ (M ↾ X).IsFiniteRankUniform (a + 1) } with h_UnifS
---   have hne : Unif.Nonempty := by
---     refine ⟨B, (IsBase.subset_ground hB), ?_, ?_,⟩
---     · rwa [eRank_restrict, hB.eRk_eq_eRank]
---     rw [hB.indep.restrict_eq_freeOn]
---     exact freeOn_uniform B
---   have hYbound : ∀ Y, Y ∈ Unif → Y.encard < b + 1 := by
---     intro X hX
---     by_contra hc
---     simp only [not_lt] at hc
---     --have : X ⊆ M.E := by exact hX.1
---     have h2 : ((unifOn (M ↾ X).E (a + 1)).NoUniformMinor (a + 1) (b + 1)) := by
---       rw[←hX.2.eq_unifOn ]
---       exact hM.minor (IsRestriction.isMinor (restrict_isRestriction M X) )
---     have h3 := unifOn_noUniformMinor_iff.1 h2
---     grw [← restrict_ground_eq (M := M) (R := X)] at hc
---     grind
---     --simp only [mem_setOf_eq] at hX
---     -- exact hc.not_gt <| hM.lt_of_isoMinor (N := M ↾ X) (b' := X.encard)
---     --   (restrict_isRestriction _ _ hX.1).isMinor.isoMinor sorry
---   have hcard : (encard '' Unif).Finite := by
---     refine ENat.finite_of_sSup_lt_top ?_
---     refine lt_of_le_of_lt ?_ <| WithTop.natCast_lt_top (b + 1)
---     simp only [sSup_le_iff, mem_image, forall_exists_index, and_imp]
---     intro k A hAE h
---     rw[←h ]
---     exact Std.le_of_lt (hYbound A ⟨hAE.1, hAE.2 ⟩ )
---   obtain ⟨X, hX⟩ := Finite.exists_maximalFor' encard _ hcard hne
---   have hXb : X.encard < b + 1 := hYbound X hX.prop
---   set Subsets : Set (Set α) := { Y | Y ⊆ X ∧ Y.encard = a} with h_sub
---   --(Set.encard_le_coe_iff.1 (ENat.lt_coe_add_one_iff.mp hXb )).1
---   have hiC := base_isCover (Std.le_of_eq hr ) ha
---       ((Set.encard_le_coe_iff.1 (ENat.lt_coe_add_one_iff.mp hXb )).1) hX
---   --have hiC : M.IsCover (fun M X ↦ M.eRk X ≤ a) (M.closure '' Subsets) := by base_isCover
---   obtain ⟨x, hx ⟩ := ENat.ne_top_iff_exists.1 (LT.lt.ne_top hXb )
---   rw[←hx] at hXb
---   grw [hiC.coverNumber_le, Set.encard_image_le, (set_to_binom_number) X hx.symm,
---     (Nat.choose_le_choose a (Nat.le_of_lt_succ (ENat.coe_lt_coe.mp hXb )))] at hcon
---   simp only [lt_self_iff_false] at hcon
-
--- lemma coverNumber_rank_Frombase {a b : ℕ} (ha : 1 ≤ a)
---     (hM : NoUniformMinor M ( a + 1 ) (b + 1)) :
---     M.coverNumber (fun M X ↦ M.eRk X ≤ a) ≤
---     (Nat.choose b a) * M.coverNumber (fun M X ↦ M.eRk X ≤ (a + 1)) := by
---   sorry
-
--- lemma coverNumber_Bound {M : Matroid α} [M.RankPos] {a b : ℕ} {n : ℕ∞} (ha : a ≠ 0) (hb : a ≤ b)
---     (hM : NoUniformMinor M ( a + 1 ) (b + 1)) (hn : M.eRank = a + n) :
---     M.coverNumber (fun M X ↦ M.eRk X ≤ a) ≤ (Nat.choose b a)^(M.eRank - a) := by
---   obtain htop | hfin := eq_or_ne M.eRank ⊤
---   · grw [htop, ENat.top_sub_coe, ENat.epow_top, ← le_top]
---     obtain rfl | hlt := hb.eq_or_lt
---     · simp [noUniformMinor_self_iff, htop] at hM
---     rw [← ENat.coe_one, ENat.coe_lt_coe]
---     suffices b.choose a ≠ 0 ∧ b.choose a ≠ 1 by lia
---     exact ⟨(Nat.choose_pos hlt.le).ne.symm, by simp [Nat.choose_eq_one_iff, hlt.ne.symm, ha]⟩
---   by_cases h0 : n = 0
---   · -- When M.eRank = a, you can cover with (M.E). This is a lemma somewhere
---     sorry
---   --Now you can assume n ≠ 0 and n - 1 makes sense
---   obtain ⟨e, heC⟩ : ∃ e, M.IsNonloop e := exists_isNonloop M
---   have h' : (M ／ {e}).eRank < M.eRank := by sorry
---   have hRP : ( M ／ {e}).RankPos := by sorry --I think here you need n ≠ 0
---   have hM' : NoUniformMinor ( M ／ {e}) ( a + 1 ) (b + 1) := by sorry
---   have hn' : (M ／ {e}).eRank = a + (n - 1) := by sorry
---   have ih := coverNumber_Bound (M := M ／ {e}) (a := a) (b := b) ha hb hM' (n := n - 1)
---   sorry
--- termination_by M.eRank
-
---   -- suffices hn : ∀ n : ℕ, M.eRank = n + a + 1 →
---   --     M.coverNumber (fun M X ↦ M.eRk X ≤ a) ≤ (Nat.choose b a)^(n + 1 )
---   -- ·
---   --   sorry
---   -- intro n hn
---   -- induction n generalizing M with
---   -- | zero => sorry
---   -- | succ n IH => sorry
-
--- -- -- change `ha` to `a ≠ 0`.
--- -- lemma coverNumber_Bound_contract [M.RankFinite] {a b : ℕ} (ha : 1 ≤ a)
--- --     (hM : NoUniformMinor M ( a + 1 ) (b + 1)) (hC : C ⊂ M.E)  :
--- --     M.coverNumber (fun M X ↦ M.eRk X ≤ a) ≤
--- --     (Nat.choose b a)^(M.eRk C ) * (M／C).coverNumber (fun M X ↦ M.eRk X ≤ a) := by
--- --   suffices hn : ∀ n : ℕ, n = M.eRk C →  M.coverNumber (fun M X ↦ M.eRk X ≤ a) ≤
--- --       (Nat.choose b a)^n * (M／C).coverNumber (fun M X ↦ M.eRk X ≤ a)
--- --   · obtain ⟨ n, hh ⟩ := ENat.ne_top_iff_exists.1 ( eRk_ne_top (M := M) (X := C))
--- --     rw[←hh]
--- --     exact le_of_eq_of_le rfl (hn n hh)
--- --   intro n hn
--- --   induction n generalizing M C with
--- --   | zero =>
--- --     simp only [pow_zero, one_mul]
--- --     rw [coverNumber_contract_loop ((ground_nonempty_iff (M ＼ C)).mp (nonempty_of_ssubset hC ) )
--- --       (ENat.one_le_coe.mpr ha ) ((eRk_eq_zero_iff (subset_of_ssubset hC)).1 hn.symm )]
--- --   | succ n IH =>
--- --   grw[coverNumber_rank_Frombase ha hM ]
--- --   have hresP : (M ↾ C).RankPos :=
--- --     (eRank_ne_zero_iff (M ↾ C)).mp <| by simp [eRank_restrict, ne_eq, ← hn]
-
--- --   obtain ⟨e, heC ⟩ := exists_isNonloop (M ↾ C)
--- --   obtain ⟨heC1, heC2 ⟩ := restrict_isNonloop_iff.1 heC
--- --   have heN : (M／ {e}).Nonempty := by
--- --     rw[←(M／ {e}).ground_nonempty_iff, contract_ground]
--- --     exact (Set.nonempty_of_ssubset (by grind ) )
--- --   grw[ coverNumber_contract_one (heC1.mem_ground ) heC1 heN]
--- --   have hn1 : (M／ {e}).eRk (C \ {e}) = n := by
--- --     have hrelrk := IsNonloop.eRelRk_add_one_eq heC1 (C \ {e})
--- --     simp only [insert_diff_singleton, insert_eq_of_mem heC2, ←hn, Nat.cast_add, Nat.cast_one,
--- --       ne_eq, ENat.one_ne_top, not_false_eq_true,
--- --       add_left_inj_of_ne_top] at hrelrk
--- --     rwa [eRelRk.eq_1] at hrelrk
--- --   have hsub1 : (C \ {e}) ⊂ (M／ {e}).E := by
--- --     simp only [contract_ground]
--- --     refine Set.ssubset_iff_subset_ne.mpr ⟨diff_subset_diff_left (subset_of_ssubset hC), ?_ ⟩
--- --     by_contra hc
--- --     have h : C = M.E := by
--- --       rw [←insert_diff_self_of_mem heC2, ←insert_diff_self_of_mem heC1.mem_ground, hc]
--- --     have hCE : C ≠ M.E := by exact Std.ne_of_lt hC
--- --     rw [h] at hCE
--- --     exact false_of_ne hCE
--- --   grw[ IH (hM.minor (contract_isMinor M {e} )) hsub1 hn1.symm ]
--- --   simp only [contract_contract, union_diff_self, singleton_union, ge_iff_le, insert_eq_of_mem heC2,
--- --     ←mul_assoc ]
--- --   nth_rw 1 [ ←ENat.epow_one (x := ↑(b.choose a)), ←ENat.epow_natCast,
--- --     ←ENat.epow_add (x :=  ↑(b.choose a)) (y := 1) (z := n ), ←ENat.coe_one, ←ENat.coe_add,
--- --     ENat.epow_natCast, add_comm ]
-
-
--- -- change `ha` to `a ≠ 0`.
--- lemma coverNumber_Bound_contract {M : Matroid α} {C : Set α} {a b : ℕ} (ha : a ≠ 0) (hb : a ≤ b)
---     (hM : NoUniformMinor M (a + 1) (b + 1)) (hC : C ⊂ M.E)  :
---     M.coverNumber (fun M X ↦ M.eRk X ≤ a) ≤
---     (Nat.choose b a)^(M.eRk C) * (M ／ C).coverNumber (fun M X ↦ M.eRk X ≤ a) := by
---   obtain htop | hlt := eq_or_ne (M.eRk C) ⊤
---   · grw [htop, ENat.epow_top, ENat.top_mul, ← le_top ]
---     · have heN : (M／ C).Nonempty := by
---         rw[←(M／ C).ground_nonempty_iff, contract_ground]
---         exact (Set.nonempty_of_ssubset (by grind ) )
---       exact ENat.one_le_iff_ne_zero.mp (coverNumer_positive (fun M X ↦ M.eRk X ≤ a) )
---     obtain rfl | hlt := hb.eq_or_lt
---     · simp [noUniformMinor_self_iff] at hM
---       grw [ ←eRk_le_eRank M C, htop ] at hM
---       simp only [not_top_lt] at hM
---     rw [← ENat.coe_one, ENat.coe_lt_coe]
---     suffices b.choose a ≠ 0 ∧ b.choose a ≠ 1 by lia
---     exact ⟨(Nat.choose_pos hlt.le).ne.symm, by simp [Nat.choose_eq_one_iff, hlt.ne.symm, ha] ⟩
---   have hresP : (M ↾ C).RankPos := sorry
---     -- (eRank_ne_zero_iff (M ↾ C)).mp <| by simp [eRank_restrict, ne_eq, ← hn]
---   obtain ⟨e, heC⟩ : ∃ e, (M ↾ C).IsNonloop e := exists_isNonloop (M ↾ C)
---   rw [restrict_isNonloop_iff] at heC
---   -- have hrelrk := IsNonloop.eRelRk_add_one_eq heC.1 (C \ {e})
---   -- simp only [insert_diff_singleton, insert_eq_of_mem heC.2] at hrelrk
---   have h' : (M ／ {e}).eRk (C \ {e}) < M.eRk C := by
---     have hrelrk := IsNonloop.eRelRk_add_one_eq heC.1 (C \ {e})
---     simp only [insert_diff_singleton, insert_eq_of_mem heC.2] at hrelrk
---     rw [ ←hrelrk, eRelRk.eq_1 ]
---     simp only [ENat.lt_add_left_iff, ne_eq, eRk_eq_top_iff, IsRkFinite.diff_singleton_iff, not_not,
---       one_ne_zero, not_false_eq_true, and_true]
---     rw [ IsRkFinite ]
---     refine eRank_lt_top_iff.mp ?_
---     grw [eRank_restrict, eRk_contract_le_eRk M {e} C]
---     exact Ne.lt_top' (id (Ne.symm hlt))
---   have hsub1 : (C \ {e}) ⊂ (M／ {e}).E := by
---     simp only [contract_ground]
---     refine Set.ssubset_iff_subset_ne.mpr ⟨diff_subset_diff_left (subset_of_ssubset hC), ?_ ⟩
---     by_contra hc
---     have h : C = M.E := by
---       rw [←insert_diff_self_of_mem heC.2, ←insert_diff_self_of_mem heC.1.mem_ground, hc]
---     grind
---   have heN : (M／ {e}).Nonempty := by
---     rw[←(M／ {e}).ground_nonempty_iff, contract_ground]
---     exact (Set.nonempty_of_ssubset (by grind ) )
---   have : 1 ≤ a := by exact Nat.one_le_iff_ne_zero.mpr ha
---   have ih := coverNumber_Bound_contract (M := M ／ {e}) (C := C \ {e}) (a := a) (b := b) ha
---     hb (hM.minor (contract_isMinor M {e} )) hsub1
---   grw [coverNumber_rank_Frombase (Nat.one_le_iff_ne_zero.mpr ha) hM, coverNumber_contract_one (heC.1.mem_ground ) heC.1 heN, ih ]
---   simp only [contract_contract, union_diff_self, singleton_union, ge_iff_le, insert_eq_of_mem heC.2,
---     ←mul_assoc]
---   nth_rw 1 [←eRelRk.eq_1, ←ENat.epow_one (x := ↑(b.choose a)),
---     ←ENat.epow_add (x :=  ↑(b.choose a)) (y := 1) (z := (M.eRelRk {e} (C \ {e})) ),
---     ←add_comm (a := (M.eRelRk {e} (C \ {e}))) (b:= 1 ), (heC.1).eRelRk_add_one_eq, insert_diff_singleton, insert_eq_of_mem heC.2 ]
-
--- termination_by M.eRk C
-
-
--- end Rank
-
--- section NonSpanning
-
--- lemma NonSpanning_to_RankCover [M.RankFinite] (hM : 2 ≤ M.eRank) :
---     M.IsCover Matroid.Nonspanning T ↔ M.IsRankCover (M.eRank - 1) T := by
---   refine ⟨?_, ?_ ⟩
---   · intro h
---     refine ⟨ h.sUnion_eq, ?_ ⟩
---     intro F hF
---     by_contra hc
---     simp only [not_le] at hc
---     have : M.eRank ≤ M.eRk F := by
---       have : M.eRank - 1 + 1 ≤  M.eRk F := by exact Order.add_one_le_of_lt hc
---       sorry
---     sorry
---   sorry
-
--- lemma NonSpaning_le_two [M.Nonempty] (hle : M.eRank ≤ 1) :
---     ⊤ ≤ M.coverNumber (Matroid.Nonspanning) := by
---   obtain hT | ⟨T, hT1, hT2 ⟩  := M.exists_cover (Matroid.Nonspanning)
---   · rw[ hT ]
---   by_contra hc
---   have : M.RankFinite := by
---     refine eRank_lt_top_iff.mp ?_
---     grw[hle]
---     exact ENat.one_lt_top
---   have hu := hT1.sUnion_eq
---   have hl : ∀ T1 ∈ T, T1 ⊆ M.loops := by
---     intro T1 hT'
---     have h1 : M.eRk T1 < M.eRank := Nonspanning.eRk_lt (hT1.pProp T1 hT' )
---     grw [hle] at h1
---     simp only [ENat.lt_one_iff] at h1
---     exact (M.eRk_eq_zero_iff (X := T1) (hX := by grind)).1 h1
---   have hs : M.E ⊆ M.loops := by
---     rw [←hT1.sUnion_eq]
---     exact sUnion_subset hl
---   obtain ⟨T', hT' ⟩ := hT1.nonempty
---   have h2 : M.E ⊆ M.closure T' := by
---     grw [hs]
---     exact loops_subset_closure M T'
---   exact Ne.elim (fun a ↦ ((hT1.pProp T' hT').not_spanning) ((spanning_iff_ground_subset_closure
---     (hT1.subset_ground hT') ).2 h2)) hT2
-
-
--- lemma Non_spanning_singleton (he : e ∈ M.E) (hM : 2 ≤ M.eRank) : M.Nonspanning {e} := by
---     by_contra hc
---     have h1 : M.eRank ≤ 1 := by
---       rw [not_nonspanning_iff] at hc
---       rw [←hc.eRk_eq]
---       simp only [eRk_singleton_le]
---     grw [←hM] at h1
---     simp only [ENat.not_ofNat_le_one] at h1
-
--- lemma IsCover_singleton_NonSpanning (hM : 2 ≤ M.eRank) :
---     M.IsCover (Matroid.Nonspanning) (singleton '' M.E) := by
---   exact IsCover_singleton_Prop (fun e he ↦ Non_spanning_singleton he hM)
-
--- lemma IsCover_singleton_le_NonSpanning (hM : 2 ≤ M.eRank) :
---     M.coverNumber (Matroid.Nonspanning) ≤ M.E.encard := by
---   exact IsCover_singleton_le (fun e he ↦ Non_spanning_singleton he hM)
-
--- lemma NonSpaning_cover_exists (hM : 2 ≤ M.eRank) : M.hasCover_with Matroid.Nonspanning := by
---   refine ⟨(singleton '' M.E), IsCover_singleton_NonSpanning hM ⟩
-
--- lemma IsNonSpaningCover_contract (h : (M ／ X).IsCover (Matroid.Nonspanning) T)
---     (hX : X ⊆ M.E) (hXN : (M ／ X).Nonempty) :
---     M.IsCover (Matroid.Nonspanning) ((· ∪ X) '' T) := by
---   apply h.contract hX hXN
---   intro Y hC
---   refine ⟨ ?_, union_subset (by have := hC.subset_ground; grind ) hX  ⟩
---   · by_contra hc
---     have hcc : (M ／ X).Spanning Y := by
---       have h1 := hc.contract X
---       simp only [union_diff_right] at h1
---       exact h1.superset (diff_subset (s := Y) (t := X)) (hC.subset_ground)
---     rw [←not_spanning_iff hcc.subset_ground ] at hC
---     exact (iff_false_intro hC).mp hcc
-
--- lemma NonSpanningNumber_contract (hX : X ⊆ M.E) (hne : (M ／ X).Nonempty) :
---     M.coverNumber Matroid.Nonspanning ≤ (M ／ X).coverNumber Matroid.Nonspanning := by
---   obtain hT | ⟨T, hT, hTe ⟩ := (M ／ X).exists_cover (Matroid.Nonspanning)
---   · rw [hT]
---     exact OrderTop.le_top (M.coverNumber Nonspanning)
---   rw [← hTe]
---   exact
---     Std.IsPreorder.le_trans (M.coverNumber Nonspanning) ((fun x ↦ x ∪ X) '' T).encard T.encard
---       ((IsNonSpaningCover_contract hT hX hne).coverNumber_le)
---       (encard_image_le (fun x ↦ x ∪ X) T )
-
--- lemma NonSpanningNumber_set_closure (hY : Y ⊆ M.closure X) (hX : X ⊆ M.E) :
---     (M ↾ X).coverNumber Nonspanning  ≤ (M ↾ (X ∪ Y)).coverNumber Nonspanning := by
---   obtain hT | ⟨T, hT, hTe ⟩ := (M ↾ (X ∪ Y)).exists_cover (Matroid.Nonspanning)
---   · rw [hT]
---     exact OrderTop.le_top ((M ↾ X).coverNumber Nonspanning)
---   rw[←hTe]
---   have hcov : (M ↾ X).IsCover (Matroid.Nonspanning) ((fun x ↦ x ∩ X) '' T) := by
---     refine ⟨?_, ?_ ⟩
---     · refine subset_antisymm (sUnion_subset fun K ↦ ?_) fun e he ↦ ?_
---       · intro hK
---         obtain ⟨K', hK'T, hK' ⟩ := hK
---         rw [← hK']
---         grind
---       have h1 := hT.sUnion_eq
---       simp only [restrict_ground_eq] at h1
---       simp only [restrict_ground_eq] at he
---       have : e ∈  ⋃₀ T := by grind
---       obtain ⟨ T', hT', heT' ⟩ := this
---       have : e ∈ T' ∩ X := by grind
---       grind
---     intro F hF
---     obtain ⟨F', hF', hhF' ⟩ := hF
---     simp only at hhF'
---     rw [← hhF']
---     by_contra hc
---     rw [not_nonspanning_iff, restrict_spanning_iff (by grind)] at hc
---     have hcc : X ∪ Y ⊆ M.closure F' := union_subset (LE.le.subset fun ⦃a⦄ a_1 ↦
---       (closure_subset_closure M (inter_subset_left )) (hc a_1)) ( LE.le.subset fun ⦃a⦄ a_1 ↦
---       (closure_subset_closure M (inter_subset_left )) ((LE.le.subset fun ⦃a⦄ a_1 ↦
---       (closure_subset_closure_of_subset_closure hc ) (hY a_1) ) a_1))
---     rw [←restrict_spanning_iff (hR := by grind), ←not_nonspanning_iff (by grind)  ] at hcc
---     exact Ne.elim (fun a ↦ hcc (hT.pProp F' hF')) hTe
---     exact LE.le.subset (hT.subset_ground hF')
---   grw [hcov.coverNumber_le ]
---   exact encard_image_le (fun x ↦ x ∩ X) T
-
-
-
--- -- lemma NonSpaningNumber_delete_loop (hne : (M ＼ D).Nonempty) (hk : 1 ≤ k) (hD : D ⊆ M.loops ) :
--- --     M.coverNumber (fun M X ↦ M.eRk X ≤ k) = (M ＼ D).coverNumber (fun M X ↦ M.eRk X ≤ k) := by
-
--- --   sorry
---   -- obtain ⟨T, hT, hTen ⟩ := exists_min_cover (RankPropCover_exists (M := M) hk )
---   -- have h1 := (hT.delete D ).coverNumber_le
---   -- grw[encard_image_le (fun s ↦ s \ D) T, hTen ] at h1
---   -- obtain ⟨T', hT', hT'en ⟩ := exists_min_cover (RankPropCover_exists (M := (M ＼ D)) hk )
---   -- have hcov : M.IsCover (fun M X ↦ M.eRk X ≤ k) (M.closure '' T' ) := by
---   --   refine ⟨ ?_, ?_ ⟩
---   --   · refine subset_antisymm (sUnion_subset fun K ↦ ?_) fun e he ↦ ?_
---   --     · simp only [mem_image, forall_exists_index, and_imp]
---   --       grind
---   --     by_cases heD : e ∈ D
---   --     · obtain ⟨ X, hX ⟩ := hT'.nonempty
---   --       have := (IsLoop.mem_closure (hD heD) X )
---   --       grind
---   --     have h2 : e ∈ M.E \ D := mem_diff_of_mem he heD
---   --     rw[←delete_ground,  ←hT'.sUnion_eq  ] at h2
---   --     obtain ⟨ X, hX, heX ⟩ := h2
---   --     have := (mem_closure_of_mem' M heX he )
---   --     grind
---   --   intro F hF
---   --   obtain ⟨F' ,hF', hF2 ⟩ := hF
---   --   rw[←hF2, eRk_closure_eq M F']
---   --   have ha := hT'.pProp F' hF'
---   --   simp only [delete_eRk_eq'] at ha
---   --   have ha1 : F' \ D = F' := by
---   --     have := hT'.subset_ground hF'
---   --     grind
---   --   rwa [ha1] at ha
---   -- have h2 := hcov.coverNumber_le
---   -- grw [encard_image_le M.closure T', hT'en] at h2
---   -- grind
-
--- -- lemma NonSpaningNumber_contract_loop (hne : (M ＼ D).Nonempty) (hk : 1 ≤ k) (hD : D ⊆ M.loops ) :
--- --     M.coverNumber (fun M X ↦ M.eRk X ≤ k) = (M ／ D).coverNumber (fun M X ↦ M.eRk X ≤ k) := by
--- --   rw[contract_eq_delete_of_subset_loops hD]
--- --   exact coverNumber_delete_loop hne hk hD
-
-
-
-
--- end NonSpanning
-
-
-
-
-
-
-
-
-
-
-
-
--- section Indexed
-
--- variable {T : ι → Set α}
-
--- @[mk_iff]
--- structure IsIndexedCover (M : Matroid α) (k : ℕ∞) (T : ι → Set α) : Prop where
---   iUnion_eq : ⋃ i, T i = M.E
---   eRk_le : ∀ i, M.eRk (T i) ≤ k
-
--- lemma IsIndexedCover.subset_ground (h : M.IsIndexedCover k T) (i : ι) : T i ⊆ M.E := by
---   grw [← h.iUnion_eq, ← subset_iUnion]
-
--- lemma IsIndexedCover.isIndexedCover_closure (h : M.IsIndexedCover k T) :
---     M.IsIndexedCover k (fun i ↦ M.closure (T i)) := by
---   refine ⟨(iUnion_subset (fun i ↦ M.closure_subset_ground ..)).antisymm ?_, fun i ↦ ?_⟩
---   · grw [← h.iUnion_eq, iUnion_mono (fun i ↦ M.subset_closure (T i) (h.subset_ground i))]
---   simpa using h.eRk_le i
-
--- lemma setOf_point_isIndexedCover (M : Matroid α) [M.RankPos] :
---     M.IsIndexedCover 1 (fun x : {P // M.IsPoint P} ↦ x.1) := by
---   refine ⟨(iUnion_subset fun P ↦ P.2.subset_ground).antisymm fun e he ↦ ?_, ?_⟩
---   · obtain hl | hnl := M.isLoop_or_isNonloop e
---     · obtain ⟨f, hf⟩ := M.exists_isNonloop
---       exact mem_iUnion_of_mem (i := ⟨M.closure {f}, hf.closure_isPoint⟩) <| hl.mem_closure {f}
---     exact mem_iUnion_of_mem (i := ⟨M.closure {e}, hnl.closure_isPoint⟩) <| M.mem_closure_self e
---   simp +contextual [IsPoint.eRk]
-
--- lemma IsIndexedCover.cover_cover {η : ι → Type*} (h : M.IsIndexedCover k T)
---     (T₀ : (i : ι) → (η i) → Set α) (hT₀ : ∀ i, (M ↾ (T i)).IsIndexedCover a (T₀ i)) :
---     M.IsIndexedCover a (fun i : ((i : ι) × η i) ↦ T₀ i.1 i.2) := by
---   refine ⟨?_, ?_⟩
---   · rw [← h.iUnion_eq, iUnion_sigma]
---     refine iUnion_congr fun i ↦ ?_
---     rw [(hT₀ i).iUnion_eq, restrict_ground_eq]
---   rintro ⟨i, j⟩
---   have := (hT₀ i).eRk_le j
---   rwa [restrict_eRk_eq', inter_eq_self_of_subset_left] at this
---   grw [(hT₀ i).subset_ground, restrict_ground_eq]
-
-
-
-
--- noncomputable def coverNumber' (M : Matroid α) (k : ℕ∞) :=
---     ⨅ (T : Set (Set α)) (_ : M.IsIndexedCover k (fun x : T ↦ x)), T.encard
-
--- lemma IsIndexedCover.coverNumber'_le {T : Set (Set α)} (hT : M.IsIndexedCover k (fun x : T ↦ x)) :
-
-
--- lemma IsIndexedCover.coverNumber'_le (h : M.IsIndexedCover k T) : M.coverNumber' k ≤ ENat.card ι := by
---   grw [coverNumber', iInf₂_le _ (i := range T)]
---   · grw [← image_univ, encard_image_le, encard_le_card]
-
-
-
-
-
--- end Indexed
-
--- def IsCover (M : Matroid α) (k : ℕ∞) (T : Set (Set α)) : Prop := M.IsIndexedCover k (fun X : T ↦ X.1)
-
--- lemma IsCover.isIndexedCover (h : M.IsCover k T) : M.IsIndexedCover k (fun X : T ↦ X.1) := h
-
--- lemma IsCover.sUnion_eq (h : M.IsCover k T) : ⋃₀ T = M.E := by
---   rw [← IsIndexedCover.iUnion_eq h, sUnion_eq_iUnion]
-
--- lemma IsCover.eRk_le (h : M.IsCover k T) (hXT : X ∈ T) : M.eRk X ≤ k :=
---   IsIndexedCover.eRk_le h ⟨X, hXT⟩
-
--- lemma isCover_iff : M.IsCover k T ↔ ⋃₀ T = M.E ∧ ∀ F ∈ T, M.eRk F ≤ k :=
---   ⟨fun h ↦ ⟨h.sUnion_eq, fun _ ↦ h.eRk_le⟩,
---     fun h ↦ ⟨by rw [← sUnion_eq_iUnion, h.1], by simpa using h.2⟩⟩
-
-
-
--- -- @[mk_iff]
--- -- structure IsCover (M : Matroid α) (k : ℕ∞) (T : Set (Set α)) : Prop where
--- --   sUnion_eq : ⋃₀ T = M.E
--- --   eRk_le : ∀ F ∈ T, M.eRk F ≤ k
-
--- lemma IsCover.subset_ground (h : M.IsCover k T) (hX : X ∈ T) : X ⊆ M.E := by
---   grw [← h.sUnion_eq, ← subset_sUnion_of_mem hX]
-
--- lemma IsCover.isCover_closure (h : M.IsCover k T) : M.IsCover k (M.closure '' T) := by
---   simp only [isCover_iff, sUnion_image, subset_antisymm_iff (b := M.E), iUnion_subset_iff,
---     M.closure_subset_ground, implies_true, true_and, mem_image, forall_exists_index, and_imp,
---     forall_apply_eq_imp_iff₂, eRk_closure_eq]
---   grw [h.sUnion_eq.symm.subset, sUnion_eq_biUnion]
---   exact ⟨biUnion_mono rfl.subset fun X hX ↦ M.subset_closure X (h.subset_ground hX),
---     fun _ ↦ h.eRk_le⟩
-
--- lemma IsCover.mono {k'} (h : M.IsCover k T) (hkk' : k ≤ k') : M.IsCover k' T :=
---   isCover_iff.2 ⟨h.sUnion_eq, fun _ hF ↦ (h.eRk_le hF).trans hkk'⟩
-
--- lemma ground_isCover (M : Matroid α) : M.IsCover M.eRank {M.E} := by
---   simp [isCover_iff]
-
--- -- lemma setOf_point_isCover (M : Matroid α) [M.RankPos] : M.IsCover 1 {P | M.IsPoint P} := by
--- --   refine ⟨subset_antisymm (sUnion_subset fun _ ↦ IsPoint.subset_ground) fun e he ↦ ?_,
--- --     by simp +contextual [mem_setOf_eq, IsPoint] ⟩
--- --   simp only [mem_sUnion, mem_setOf_eq]
--- --   obtain hl | hnl := M.isLoop_or_isNonloop e
--- --   · obtain ⟨f, hf⟩ := M.exists_isNonloop
--- --     exact ⟨_, hf.closure_isPoint, hl.mem_closure _⟩
--- --   exact ⟨_, hnl.closure_isPoint, mem_closure_of_mem _ (by simp) (by simpa)⟩
-
--- -- lemma setOf_point_IsCover [hM : M.Loopless] : M.IsCover 1 {P | M.IsPoint P} := by
--- --   obtain ⟨E, rfl⟩ | h := M.eq_loopyOn_or_rankPos'
--- --   · obtain rfl : E = ∅ := by simpa using hM
--- --     constructor <;> simp [IsPoint]
--- --   exact M.setOf_point_isCover
-
-
--- -- lemma IsCover.contract (h : (M ／ X).IsCover k T) (hX : X ⊆ M.E) (hXN : (M ／ X).Nonempty) :
--- --     M.IsCover (k + M.eRk X) ((· ∪ X) '' T) := by
--- --   suffices ∀ F ∈ T, M.eRk (F ∪ X) ≤ k + M.eRk X by
--- --     simpa [isCover_iff, ← biUnion_distrib_union _ h.nonempty, ← sUnion_eq_biUnion, h.sUnion_eq, hX]
--- --   exact fun F hFT ↦ by grw [← h.eRk_le F hFT, ← eRelRk_eq_eRk_contract, eRelRk_add_eRk_eq]
-
--- /-- The number of sets of rank at most `k` needed to cover a matroid `M`. -/
--- noncomputable def coverNumber (M : Matroid α) (k : ℕ∞) : ℕ∞ := sInf (encard '' {T | M.IsCover k T})
-
--- lemma coverNumber_eq_iInf (M : Matroid α) (k : ℕ∞) :
---     M.coverNumber k = ⨅ T ∈ {T | M.IsCover k T}, T.encard := by
---   exact sInf_image
-
--- lemma IsCover.coverNumber_le (h : M.IsCover k T) : M.coverNumber k ≤ T.encard :=
---   sInf_le <| by grind
-
--- @[simp]
--- lemma coverNumber_emptyOn (α : Type*) (k : ℕ∞) : (emptyOn α).coverNumber k = 0 := by
---   simp [coverNumber, ENat.sInf_eq_zero, isCover_iff]
-
--- lemma coverNumber_pos (M : Matroid α) [M.Nonempty] (k : ℕ∞) : 0 < M.coverNumber k := by
---   suffices ¬ M.IsCover k ∅ by simpa [pos_iff_ne_zero, coverNumber, ENat.sInf_eq_zero]
---   exact fun h ↦ M.ground_nonempty.ne_empty <| by simpa using h.sUnion_eq.symm
-
--- @[simp]
--- lemma coverNumber_top (M : Matroid α) [M.Nonempty] : M.coverNumber ⊤ = 1 := by
---   nth_grw 1 [le_antisymm_iff, ENat.one_le_iff_ne_zero,
---     (M.ground_isCover.mono (by simp)).coverNumber_le, encard_singleton, and_iff_right rfl.le]
---   exact (M.coverNumber_pos _).ne.symm
-
--- lemma coverNumber_le {k k' : ℕ∞} (M : Matroid α) (hk : k ≤ k') : M.coverNumber k' ≤ M.coverNumber k
---     := by
---   refine ENat.forall_natCast_le_iff_le.mp ?_
---   intro a hak
---   unfold coverNumber at hak
---   simp only [le_sInf_iff, mem_image, mem_setOf_eq, forall_exists_index, and_imp,
---     forall_apply_eq_imp_iff₂] at hak
---   unfold coverNumber
---   simp only [le_sInf_iff, mem_image, mem_setOf_eq, forall_exists_index, and_imp,
---     forall_apply_eq_imp_iff₂]
---   exact fun T hT ↦ (hak T (hT.mono hk))
-
--- lemma coverNumber_contract_one {a : ℕ∞} (he : e ∈ M.E) (hel : M.IsNonloop e)
---     (heN : (M／ {e}).Nonempty) :
---     M.coverNumber (a + 1) ≤ (M ／ {e}).coverNumber a := by
---   refine ENat.forall_natCast_le_iff_le.mp ?_
---   intro b hb
---   unfold coverNumber at hb
---   simp only [le_sInf_iff, mem_image, mem_setOf_eq, forall_exists_index, and_imp,
---     forall_apply_eq_imp_iff₂] at hb
---   unfold coverNumber
---   simp only [le_sInf_iff, mem_image, mem_setOf_eq, forall_exists_index, and_imp,
---     forall_apply_eq_imp_iff₂]
---   intro T hT
---   have h1 := hT.contract (singleton_subset_iff.mpr he ) heN
---   rw[IsNonloop.eRk_eq hel ] at h1
---   have h2 := hb ((· ∪ {e}) '' T) h1
---   grw[encard_image_le (fun x ↦ x ∪ {e}) T ] at h2
---   exact h2
-
--- -- lemma exists_cover (M : Matroid α) {k : ℕ∞} (hk : 1 ≤ k) :
--- --     ∃ T, M.IsCover k T ∧ T.encard = M.coverNumber k := by
--- --   simpa using csInf_mem <| (M.setOf_cover_nonempty hk).image encard
-
-
-
--- lemma coverNumber_contract {a : ℕ∞} (hX : X ⊆ M.E) :
---     M.coverNumber (a + M.eRk X) ≤ (M ／ X).coverNumber a := by
---   --Mathieu, do you want to do this one?
---   sorry
-
-
--- lemma coverNumber_lt {k l : ℕ∞} (hlt : M.coverNumber k < l) : ∃ T, M.IsCover k T ∧ T.encard < l :=
---     by
--- obtain ⟨t, ⟨T, hT, hT1 ⟩, htl ⟩ := sInf_lt_iff.1 hlt
--- refine ⟨T, ⟨hT , (lt_of_eq_of_lt hT1 htl ) ⟩⟩
-
-
-    --(hcovNum : M.coverNumber a ≤ )
-
--- lemma foo (M : Matroid α) [RankPos M] : M.coverNumber 1 = M.simplification.E.encard := by
-
---   rw [M.simplification_isSimplification.encard_ground_eq, le_antisymm_iff]
---   refine ⟨M.setOf_point_isCover.coverNumber_le, ?_⟩
---   rw [coverNumber, le_sInf_iff]
---   simp
-
-
--- lemma foo (M : Matroid α) (C : Set α)
-
-
-
--- def coverNumber (M : Matroid α) (k : ℕ∞) : ℕ∞ :=
---   sInf {}
-
-  -- refine ⟨subset_antisymm (sUnion_subset fun X hX ↦ ?_) ?_, ?_⟩
-  -- ·
-
--- /-- A cover of the elements of `M` with sets of rank at most `k`. -/
--- structure Cover (M : Matroid α) (k : ℕ∞) where
---   toSet : Set (Set α)
---   sUnion_eq' : ⋃₀ toSet = M.E
---   eRk_le' : ∀ F ∈ toSet, M.eRk F ≤ k
-
--- -- `M.Cover k` behaves like a `Set` of `Set α`.
--- instance {k} : SetLike (M.Cover k) (Set α) where
---   coe := Cover.toSet
---   coe_injective' C C' _ := by cases C; cases C'; simpa
-
--- variable {T : M.Cover k}
-
--- @[simp]
--- lemma Cover.sUnion_eq (T : M.Cover k) : ⋃₀ T = M.E := T.sUnion_eq'
--- lemma Cover.eRk_le {T : M.Cover k} (h : F ∈ T) : M.eRk F ≤ k := T.eRk_le' F h
--- @[simp]
--- lemma Cover.toSet_eq_coe (T : M.Cover k) : T.toSet = T := rfl
-
--- lemma Cover.subset_ground_of_mem (hFC : F ∈ T) : F ⊆ M.E := by
---   grw [← T.sUnion_eq]
---   exact subset_sUnion_of_mem hFC
-
--- def Cover.closures (T : M.Cover k) : M.Cover k where
---   toSet := M.closure '' T
---   sUnion_eq' := by
---     refine subset
---   eRk_le' := _
-
-
--- lemma IsNonloop.contraction_points (he : M.IsNonloop e ) :
---         M.simplification.E.encard = (∑ M.IsLine L ∧ e ∈ L, L.encard) + 1
-
--- theorem kung_bound [RankFinite M]
---     (hNoUnif : NoUniformMinor M (l + 2) 2) :
---     --(hNoUnif : ∀ N : Matroid α, N ≤m M → N = (unifOn (N.E ) 2 ) → N.E.encard < l + 2) :
---     --(hNoUnif : ¬ Nonempty ((unifOn (Set.univ : Set (Fin (l + 2))) 2) ≤i M)) :
---     coverNumber M 1 ≤ ∑' i : {i : ℕ // i < M.eRank}, l^i.1  := by
---     --M.simplification.E.encard ≤ (l ^ (M.rank ) - 1)/(l - 1) := by
---   suffices hn : ∀ n : ℕ, M.rank = n → coverNumber M 1 ≤  ∑' i : {i : ℕ // i < n}, l^i.1
---   ·
---     sorry
---   intro n hn
---   sorry
---   -- I think we just need to use coverNumber_contract_one
-
-
--- def kung_infinite (hM : M.NoUniformMinor 2 (l + 2)) :
---     M.simplification.E.encard ≤ ∑' i : {i : ℕ // i < M.eRank}, l ^ i.1 := by
---   sorry
